Congruence_Closure_Explain/CC_Invars.thy
@@ -9,34 +9,34 @@ paragraph \<open>Invariants after a step in the loop\<close>
 
 lemma lookup_invar_loop2:
   assumes "lookup_invar \<lparr>cc_list = l, use_list = u, lookup = t, pending = pe, proof_forest = pf, pf_labels = pfl, input = ip\<rparr>"
-(is "lookup_invar ?base")  
-"u1 = (F a\<^sub>1 a\<^sub>2 \<approx> aa)"
-  "a\<^sub>1 < length l" "a\<^sub>2 < length l" "aa < length l"
-shows
-"lookup_invar \<lparr>cc_list = l, use_list = u[rep_b := u1 # u ! rep_b], lookup = update_lookup t l u1,
+    (is "lookup_invar ?base")  
+    "u1 = (F a\<^sub>1 a\<^sub>2 \<approx> aa)"
+    "a\<^sub>1 < length l" "a\<^sub>2 < length l" "aa < length l"
+  shows
+    "lookup_invar \<lparr>cc_list = l, use_list = u[rep_b := u1 # u ! rep_b], lookup = update_lookup t l u1,
              pending = pe, proof_forest = pf, pf_labels = pfl, input = ip\<rparr>" 
-(is "lookup_invar ?step")  
+    (is "lookup_invar ?step")  
   unfolding lookup_invar_def
 proof(standard, standard, standard, standard, standard, standard)
   fix i j
   assume i_j: "i < nr_vars ?step" "j < nr_vars ?step"
-"cc_list ?step ! i = i \<and> cc_list ?step ! j = j"
+    "cc_list ?step ! i = i \<and> cc_list ?step ! j = j"
   show "lookup_valid_element (lookup ?step) (cc_list ?step) i j"
-proof(cases "rep_of l a\<^sub>1 = i \<and> rep_of l a\<^sub>2 = j")
-  case True
-  with assms i_j nth_list_update_eq nth_update_invalid show ?thesis 
-    unfolding congruence_closure.select_convs lookup_invar_def assms(2) update_lookup.simps
-    by (smt (verit, best))
-next
-  case False
-  then have "lookup ?base ! i ! j = lookup ?step ! i ! j" 
-    using assms(2) update_lookup_unchanged by force
-  from i_j assms have "lookup_valid_element (update_lookup t l u1) l i j" 
-    unfolding lookup_invar_def congruence_closure.select_convs
-    using False update_lookup_unchanged by presburger
-  with assms show ?thesis unfolding lookup_invar_def congruence_closure.select_convs
-    by blast
-qed
+  proof(cases "rep_of l a\<^sub>1 = i \<and> rep_of l a\<^sub>2 = j")
+    case True
+    with assms i_j nth_list_update_eq nth_update_invalid show ?thesis 
+      unfolding congruence_closure.select_convs lookup_invar_def assms(2) update_lookup.simps
+      by (smt (verit, best))
+  next
+    case False
+    then have "lookup ?base ! i ! j = lookup ?step ! i ! j" 
+      using assms(2) update_lookup_unchanged by force
+    from i_j assms have "lookup_valid_element (update_lookup t l u1) l i j" 
+      unfolding lookup_invar_def congruence_closure.select_convs
+      using False update_lookup_unchanged by presburger
+    with assms show ?thesis unfolding lookup_invar_def congruence_closure.select_convs
+      by blast
+  qed
 next
   from assms show "quadratic_table (lookup ?step)"
     unfolding lookup_invar_def congruence_closure.select_convs
@@ -45,15 +45,15 @@ qed
 
 lemma use_list_invar_loop2:
   assumes "use_list_invar \<lparr>cc_list = l, use_list = u, lookup = t, pending = pe, proof_forest = pf, pf_labels = pfl, input = ip\<rparr>"
-(is "use_list_invar ?base")  
-"u1 = (F a\<^sub>1 a\<^sub>2 \<approx> aa)"
-  "a\<^sub>1 < length l" "a\<^sub>2 < length l" "aa < length l"
-"rep_b < length u"
-"rep_of l a\<^sub>1 = rep_b \<or> rep_of l a\<^sub>2 = rep_b" 
-shows
-"use_list_invar \<lparr>cc_list = l, use_list = u[rep_b := u1 # u ! rep_b], lookup = update_lookup t l u1,
+    (is "use_list_invar ?base")  
+    "u1 = (F a\<^sub>1 a\<^sub>2 \<approx> aa)"
+    "a\<^sub>1 < length l" "a\<^sub>2 < length l" "aa < length l"
+    "rep_b < length u"
+    "rep_of l a\<^sub>1 = rep_b \<or> rep_of l a\<^sub>2 = rep_b" 
+  shows
+    "use_list_invar \<lparr>cc_list = l, use_list = u[rep_b := u1 # u ! rep_b], lookup = update_lookup t l u1,
              pending = pe, proof_forest = pf, pf_labels = pfl, input = ip\<rparr>" 
-(is "use_list_invar ?step")  
+    (is "use_list_invar ?step")  
   unfolding use_list_invar_def
 proof(standard, standard, standard, standard, standard)
   fix i j
@@ -85,16 +85,16 @@ qed
 
 lemma pending_invar_loop1:
   assumes "pending_invar \<lparr>cc_list = l, use_list = u, lookup = t, pending = pe, proof_forest = pf, pf_labels = pfl, input = ip\<rparr>"
-(is "pending_invar ?base")  
-"lookup_invar \<lparr>cc_list = l, use_list = u, lookup = t, pending = pe, proof_forest = pf, pf_labels = pfl, input = ip\<rparr>"
-"u1 = (F a\<^sub>1 a\<^sub>2 \<approx> aa)"
-  "a\<^sub>1 < length l" "a\<^sub>2 < length l" "aa < length l"
-"lookup_Some t l u1" "ufa_invar l"
-shows
-"pending_invar \<lparr>cc_list = l, use_list = u, lookup = t, 
+    (is "pending_invar ?base")  
+    "lookup_invar \<lparr>cc_list = l, use_list = u, lookup = t, pending = pe, proof_forest = pf, pf_labels = pfl, input = ip\<rparr>"
+    "u1 = (F a\<^sub>1 a\<^sub>2 \<approx> aa)"
+    "a\<^sub>1 < length l" "a\<^sub>2 < length l" "aa < length l"
+    "lookup_Some t l u1" "ufa_invar l"
+  shows
+    "pending_invar \<lparr>cc_list = l, use_list = u, lookup = t, 
             pending = link_to_lookup t l u1#pe,
             proof_forest = pf, pf_labels = pfl, input = ip\<rparr>" 
-(is "pending_invar ?step")  
+    (is "pending_invar ?step")  
   unfolding pending_invar_def
 proof(standard)+
   fix i j
@@ -111,7 +111,7 @@ proof(standard)+
         apply (metis is_none_simps(1) lookup_Some.simps(1))
       by (simp_all add: assms rep_of_min)
     with assms obtain c\<^sub>1 c\<^sub>2 c where "lookup_entry t l a\<^sub>1 a\<^sub>2 = Some (F c\<^sub>1 c\<^sub>2 \<approx> c)" and
-"c\<^sub>1 < length l" "c\<^sub>2 < length l" "c < length l" "rep_of l a\<^sub>1 = rep_of l c\<^sub>1 \<and> rep_of l a\<^sub>2 = rep_of l c\<^sub>2"
+      "c\<^sub>1 < length l" "c\<^sub>2 < length l" "c < length l" "rep_of l a\<^sub>1 = rep_of l c\<^sub>1 \<and> rep_of l a\<^sub>2 = rep_of l c\<^sub>2"
       unfolding lookup_invar_def congruence_closure.select_convs
       by (metis rep_of_less_length_l)
     with 0 ** show ?thesis 
@@ -119,18 +119,19 @@ proof(standard)+
       by simp
   next
     case (Suc nat)
-then have "pending ?step ! i = pending ?base ! (i - 1)"
+    then have "pending ?step ! i = pending ?base ! (i - 1)"
       by simp
     then show ?thesis using assms unfolding pending_invar_def 
       using Suc i_j by force
   qed
 qed
 
+
 lemma inv2_loop1:
   assumes "lookup_invar \<lparr>cc_list = l, use_list = u, lookup = t, pending = pe, proof_forest = pf, 
 pf_labels = pfl, input = ip\<rparr>"
- "ufa_invar l" "lookup_Some t l u1"
-"u1 = (F a\<^sub>1 a\<^sub>2 \<approx> a)" "a\<^sub>1 < length l" "a\<^sub>2 < length l" 
+    "ufa_invar l" "lookup_Some t l u1"
+    "u1 = (F a\<^sub>1 a\<^sub>2 \<approx> a)" "a\<^sub>1 < length l" "a\<^sub>2 < length l" 
   shows "Congruence_Closure
      (representativeE
        \<lparr>cc_list = l, use_list = u, lookup = t, pending = pe, proof_forest = pf, pf_labels = pfl,
@@ -143,17 +144,17 @@ Congruence_Closure
        pending_set
         (link_to_lookup t l u1 # pe) \<union>
        set urest)"
-(is "Congruence_Closure ?base = Congruence_Closure ?step")
+    (is "Congruence_Closure ?base = Congruence_Closure ?step")
 proof-
   from assms have entry_not_none: "t ! rep_of l a\<^sub>1 ! rep_of l a\<^sub>2 \<noteq> None" 
-        by (metis is_none_simps(1) lookup_Some.simps(1))
-have "l ! rep_of l a\<^sub>1 = rep_of l a\<^sub>1 \<and> l ! rep_of l a\<^sub>2 = rep_of l a\<^sub>2"
- "rep_of l a\<^sub>1 < length l \<and> rep_of l a\<^sub>2 < length l"
-    apply (simp add: assms(2) assms(5) assms(6) rep_of_min)
+    by (metis is_none_simps(1) lookup_Some.simps(1))
+  have "l ! rep_of l a\<^sub>1 = rep_of l a\<^sub>1 \<and> l ! rep_of l a\<^sub>2 = rep_of l a\<^sub>2"
+    "rep_of l a\<^sub>1 < length l \<and> rep_of l a\<^sub>2 < length l"
+     apply (simp add: assms(2) assms(5) assms(6) rep_of_min)
     by (simp add: assms(2) assms(5) assms(6) rep_of_less_length_l)
   with assms entry_not_none 
   obtain c\<^sub>1 c\<^sub>2 c where entry: "lookup_entry t l a\<^sub>1 a\<^sub>2 = Some (F c\<^sub>1 c\<^sub>2 \<approx> c)" 
-"c\<^sub>1 < length l" "c\<^sub>2 < length l" "c < length l" "rep_of l a\<^sub>1 = rep_of l c\<^sub>1 \<and> rep_of l a\<^sub>2 = rep_of l c\<^sub>2"
+    "c\<^sub>1 < length l" "c\<^sub>2 < length l" "c < length l" "rep_of l a\<^sub>1 = rep_of l c\<^sub>1 \<and> rep_of l a\<^sub>2 = rep_of l c\<^sub>2"
     unfolding lookup_invar_def congruence_closure.select_convs 
     by metis
   from entry CC_lookup_entry_in_CC 
@@ -166,53 +167,53 @@ have "l ! rep_of l a\<^sub>1 = rep_of l a\<^sub>1 \<and> l ! rep_of l a\<^sub>2 
   have f2': "Congruence_Closure ?step (F c\<^sub>1 c\<^sub>2 \<approx> c)" using base assms(4) 
     by (metis Congruence_Closure_union \<open>l ! rep_of l a\<^sub>1 = rep_of l a\<^sub>1 \<and> l ! rep_of l a\<^sub>2 = rep_of l a\<^sub>2\<close> \<open>rep_of l a\<^sub>1 < length l \<and> rep_of l a\<^sub>2 < length l\<close> congruence_closure.select_convs(1) congruence_closure.select_convs(3))
   from entry CC_same_rep have a_c: "Congruence_Closure ?base (a\<^sub>1 \<approx> c\<^sub>1)"
-"Congruence_Closure ?base (a\<^sub>2 \<approx> c\<^sub>2)" 
+    "Congruence_Closure ?base (a\<^sub>2 \<approx> c\<^sub>2)" 
     by (metis Congruence_Closure_union assms(5,6) congruence_closure.select_convs(1))+
-from entry CC_same_rep have c_a: "Congruence_Closure ?step (c\<^sub>1 \<approx> a\<^sub>1)" 
-"Congruence_Closure ?step (c\<^sub>2 \<approx> a\<^sub>2)" 
-  by (metis Congruence_Closure_union assms(5,6) congruence_closure.select_convs(1))+
-have "u1 \<in> ?base"
-      by simp
-    have *: "u1 \<in> ?base"
-      by simp
+  from entry CC_same_rep have c_a: "Congruence_Closure ?step (c\<^sub>1 \<approx> a\<^sub>1)" 
+    "Congruence_Closure ?step (c\<^sub>2 \<approx> a\<^sub>2)" 
+    by (metis Congruence_Closure_union assms(5,6) congruence_closure.select_convs(1))+
+  have "u1 \<in> ?base"
+    by simp
+  have *: "u1 \<in> ?base"
+    by simp
   then have f1: "Congruence_Closure ?base (F a\<^sub>1 a\<^sub>2 \<approx> a)" using * base assms(4)
     by simp
   show ?thesis 
-proof(rule Congruence_Closure_eq)
-  fix eq
+  proof(rule Congruence_Closure_eq)
+    fix eq
 
 
-  assume "eq \<in> ?step"
-  then consider
-(rep) c where "eq = c \<approx> rep_of l c" "c < length l" "l ! c \<noteq> c"
-| (lookup) a' b' c c\<^sub>1 c\<^sub>2 where "eq = F a' b' \<approx> rep_of l c" "a' < length l" "b' < length l"
-"c < length l" "l ! a' = a'" "l ! b' = b'" "t ! a' ! b' = Some (F c\<^sub>1 c\<^sub>2 \<approx> c)"
-| (pending) "eq \<in> pending_set pe"
-| (new_pending) "eq \<in> pending_set [link_to_lookup t l u1]"
-| (urest) "eq \<in> set urest"
-    unfolding representativeE_def using pending_set_union
-    by fastforce
-  then show "Congruence_Closure ?base eq"
-  proof(cases)
-    case new_pending
-    
-  with new_pending assms(4) entry have eq: "eq = a \<approx> c" 
-    by auto
-  with eq f1 f2 a_c monotonic show ?thesis 
-    by simp
-  qed (simp_all add: base representativeE_def)
-next
-  fix eq' 
-  assume  "eq' \<in> ?base"
-then consider
-(rep) c where "eq' = c \<approx> rep_of l c" "c < length l" "l ! c \<noteq> c"
-| (lookup) a' b' c c\<^sub>1 c\<^sub>2 where "eq' = F a' b' \<approx> rep_of l c" "a' < length l" "b' < length l"
-"c < length l" "l ! a' = a'" "l ! b' = b'" "t ! a' ! b' = Some (F c\<^sub>1 c\<^sub>2 \<approx> c)"
-| (pending) "eq' \<in> pending_set pe"
-| (new_pending) "eq' = u1"
-| (urest) "eq' \<in> set urest" 
-  unfolding representativeE_def congruence_closure.select_convs
-  by fastforce
+    assume "eq \<in> ?step"
+    then consider
+      (rep) c where "eq = c \<approx> rep_of l c" "c < length l" "l ! c \<noteq> c"
+    | (lookup) a' b' c c\<^sub>1 c\<^sub>2 where "eq = F a' b' \<approx> rep_of l c" "a' < length l" "b' < length l"
+      "c < length l" "l ! a' = a'" "l ! b' = b'" "t ! a' ! b' = Some (F c\<^sub>1 c\<^sub>2 \<approx> c)"
+    | (pending) "eq \<in> pending_set pe"
+    | (new_pending) "eq \<in> pending_set [link_to_lookup t l u1]"
+    | (urest) "eq \<in> set urest"
+      unfolding representativeE_def using pending_set_union
+      by fastforce
+    then show "Congruence_Closure ?base eq"
+    proof(cases)
+      case new_pending
+
+      with new_pending assms(4) entry have eq: "eq = a \<approx> c" 
+        by auto
+      with eq f1 f2 a_c monotonic show ?thesis 
+        by simp
+    qed (simp_all add: base representativeE_def)
+  next
+    fix eq' 
+    assume  "eq' \<in> ?base"
+    then consider
+      (rep) c where "eq' = c \<approx> rep_of l c" "c < length l" "l ! c \<noteq> c"
+    | (lookup) a' b' c c\<^sub>1 c\<^sub>2 where "eq' = F a' b' \<approx> rep_of l c" "a' < length l" "b' < length l"
+      "c < length l" "l ! a' = a'" "l ! b' = b'" "t ! a' ! b' = Some (F c\<^sub>1 c\<^sub>2 \<approx> c)"
+    | (pending) "eq' \<in> pending_set pe"
+    | (new_pending) "eq' = u1"
+    | (urest) "eq' \<in> set urest" 
+      unfolding representativeE_def congruence_closure.select_convs
+      by fastforce
     then show "Congruence_Closure ?step eq'"
     proof(cases)
       case pending
@@ -231,8 +232,8 @@ qed
 lemma inv2_loop2:
   assumes "lookup_invar \<lparr>cc_list = l, use_list = u, lookup = t, pending = pe, proof_forest = pf, 
 pf_labels = pfl, input = ip\<rparr>" "length l = length t"
- "ufa_invar l" "\<not> lookup_Some t l u1"
-"u1 = (F a\<^sub>1 a\<^sub>2 \<approx> a)" "a\<^sub>1 < length l" "a\<^sub>2 < length l" "a < length l" 
+    "ufa_invar l" "\<not> lookup_Some t l u1"
+    "u1 = (F a\<^sub>1 a\<^sub>2 \<approx> a)" "a\<^sub>1 < length l" "a\<^sub>2 < length l" "a < length l" 
   shows "Congruence_Closure
      (representativeE
        \<lparr>cc_list = l, use_list = u, lookup = t, pending = pe, proof_forest = pf, pf_labels = pfl,
@@ -243,20 +244,20 @@ Congruence_Closure
                 lookup = update_lookup t l u1, pending = pe, proof_forest = pf, pf_labels = pfl,
                 input = ip\<rparr> \<union>
       pending_set pe \<union> set urest) "
-(is "Congruence_Closure ?base = Congruence_Closure ?step")
+    (is "Congruence_Closure ?base = Congruence_Closure ?step")
 proof(rule Congruence_Closure_eq)
   fix eq
   assume "eq \<in> ?step"
   then consider
-(rep) c where "eq = c \<approx> rep_of l c" "c < length l" "l ! c \<noteq> c"
-| (lookup) a' b' c c\<^sub>1 c\<^sub>2 where "eq = F a' b' \<approx> rep_of l c" "a' < length l" "b' < length l"
-"c < length l" "l ! a' = a'" "l ! b' = b'" "update_lookup t l u1 ! a' ! b' = Some (F c\<^sub>1 c\<^sub>2 \<approx> c)"
-"\<not> (a' = rep_of l a\<^sub>1 \<and> b' = rep_of l a\<^sub>2)"
-| (new_lookup) a' b' c c\<^sub>1 c\<^sub>2 where "eq = F a' b' \<approx> rep_of l c" "a' < length l" "b' < length l"
-"c < length l" "l ! a' = a'" "l ! b' = b'" "update_lookup t l u1 ! a' ! b' = Some (F c\<^sub>1 c\<^sub>2 \<approx> c)"
-"a' = rep_of l a\<^sub>1 \<and> b' = rep_of l a\<^sub>2"
-| (pending) "eq \<in> pending_set pe"
-| (urest) "eq \<in> set urest"
+    (rep) c where "eq = c \<approx> rep_of l c" "c < length l" "l ! c \<noteq> c"
+  | (lookup) a' b' c c\<^sub>1 c\<^sub>2 where "eq = F a' b' \<approx> rep_of l c" "a' < length l" "b' < length l"
+    "c < length l" "l ! a' = a'" "l ! b' = b'" "update_lookup t l u1 ! a' ! b' = Some (F c\<^sub>1 c\<^sub>2 \<approx> c)"
+    "\<not> (a' = rep_of l a\<^sub>1 \<and> b' = rep_of l a\<^sub>2)"
+  | (new_lookup) a' b' c c\<^sub>1 c\<^sub>2 where "eq = F a' b' \<approx> rep_of l c" "a' < length l" "b' < length l"
+    "c < length l" "l ! a' = a'" "l ! b' = b'" "update_lookup t l u1 ! a' ! b' = Some (F c\<^sub>1 c\<^sub>2 \<approx> c)"
+    "a' = rep_of l a\<^sub>1 \<and> b' = rep_of l a\<^sub>2"
+  | (pending) "eq \<in> pending_set pe"
+  | (urest) "eq \<in> set urest"
     unfolding representativeE_def using pending_set_union
     by force
   then show "Congruence_Closure ?base eq"
@@ -273,7 +274,7 @@ proof(rule Congruence_Closure_eq)
   next
     case new_lookup
     from assms have "length t = length l " "length (t ! a') = length l" 
-      apply simp using assms new_lookup(2) unfolding lookup_invar_def by auto
+       apply simp using assms new_lookup(2) unfolding lookup_invar_def by auto
     with new_lookup have lookup_entry: "update_lookup t l u1 ! a' ! b' = Some (F a\<^sub>1 a\<^sub>2 \<approx> a)"
       unfolding assms(5) update_lookup.simps  
       by fastforce
@@ -283,101 +284,746 @@ proof(rule Congruence_Closure_eq)
       using lookup_entry new_lookup(7) by simp
     with new_lookup(8,4) a_eq_rep_of_a_in_CC assms(6,7)
     have cc2: "Congruence_Closure ?base (a\<^sub>1 \<approx> a')" "Congruence_Closure ?base (a\<^sub>2 \<approx> b')" 
- "Congruence_Closure ?base (c \<approx> rep_of l c)" 
-  by (metis Congruence_Closure_union congruence_closure.select_convs(1))+
-then have "Congruence_Closure ?base (F a' b' \<approx> c)" using assms(5)
-  by (metis \<open>c = a\<close> cc1 transitive3)
+      "Congruence_Closure ?base (c \<approx> rep_of l c)" 
+      by (metis Congruence_Closure_union congruence_closure.select_convs(1))+
+    then have "Congruence_Closure ?base (F a' b' \<approx> c)" using assms(5)
+      by (metis \<open>c = a\<close> cc1 transitive3)
     then show ?thesis 
       using cc2(3) new_lookup(1) transitive2 by blast
   qed (simp_all add: base representativeE_def)
 next
   fix eq' 
   assume  "eq' \<in> ?base"
-then consider
-(rep) c where "eq' = c \<approx> rep_of l c" "c < length l" "l ! c \<noteq> c"
-| (lookup) a' b' c c\<^sub>1 c\<^sub>2 where "eq' = F a' b' \<approx> rep_of l c" "a' < length l" "b' < length l"
-"c < length l" "l ! a' = a'" "l ! b' = b'" "t ! a' ! b' = Some (F c\<^sub>1 c\<^sub>2 \<approx> c)"
-"\<not> (a' = rep_of l a\<^sub>1 \<and> b' = rep_of l a\<^sub>2)"
-| (new_lookup) a' b' c c\<^sub>1 c\<^sub>2 where "eq' = F a' b' \<approx> rep_of l c" "a' < length l" "b' < length l"
-"c < length l" "l ! a' = a'" "l ! b' = b'" "t ! a' ! b' = Some (F c\<^sub>1 c\<^sub>2 \<approx> c)"
-"a' = rep_of l a\<^sub>1 \<and> b' = rep_of l a\<^sub>2"
-| (pending) "eq' \<in> pending_set pe"
-| (new_pending) "eq' = u1"
-| (urest) "eq' \<in> set urest" 
-  unfolding representativeE_def congruence_closure.select_convs
-  by force
-    then show "Congruence_Closure ?step eq'"
-    proof(cases)
+  then consider
+    (rep) c where "eq' = c \<approx> rep_of l c" "c < length l" "l ! c \<noteq> c"
+  | (lookup) a' b' c c\<^sub>1 c\<^sub>2 where "eq' = F a' b' \<approx> rep_of l c" "a' < length l" "b' < length l"
+    "c < length l" "l ! a' = a'" "l ! b' = b'" "t ! a' ! b' = Some (F c\<^sub>1 c\<^sub>2 \<approx> c)"
+    "\<not> (a' = rep_of l a\<^sub>1 \<and> b' = rep_of l a\<^sub>2)"
+  | (new_lookup) a' b' c c\<^sub>1 c\<^sub>2 where "eq' = F a' b' \<approx> rep_of l c" "a' < length l" "b' < length l"
+    "c < length l" "l ! a' = a'" "l ! b' = b'" "t ! a' ! b' = Some (F c\<^sub>1 c\<^sub>2 \<approx> c)"
+    "a' = rep_of l a\<^sub>1 \<and> b' = rep_of l a\<^sub>2"
+  | (pending) "eq' \<in> pending_set pe"
+  | (new_pending) "eq' = u1"
+  | (urest) "eq' \<in> set urest" 
+    unfolding representativeE_def congruence_closure.select_convs
+    by force
+  then show "Congruence_Closure ?step eq'"
+  proof(cases)
     case lookup
-      then have "update_lookup t l u1 ! a' ! b' = t ! a' ! b'"
+    then have "update_lookup t l u1 ! a' ! b' = t ! a' ! b'"
       by (metis assms(5) lookup(8) update_lookup_unchanged)
     with lookup show ?thesis unfolding representativeE_def congruence_closure.select_convs
       using Congruence_Closure_split_rule mem_Collect_eq by fastforce
-    next
-      case new_lookup
-      then have "lookup_Some t l u1" 
-        by (simp add: assms(5))
-      with assms(4) have "False" 
-        by simp
-      then show ?thesis by simp
-    next
-      case new_pending
-      with assms have "length t = length l " "length (t ! rep_of l a\<^sub>1) = length l" 
-      apply simp using assms rep_of_less_length_l unfolding lookup_invar_def 
-        by fastforce
-      with assms(5) have "lookup_entry (update_lookup t l u1) l a\<^sub>1 a\<^sub>2 = Some u1" 
-        by (simp add: assms(3) assms(6) assms(7) rep_of_less_length_l)
-      with assms have "(F (rep_of l a\<^sub>1) (rep_of l a\<^sub>2) \<approx> rep_of l a) \<in> representativeE
+  next
+    case new_lookup
+    then have "lookup_Some t l u1" 
+      by (simp add: assms(5))
+    with assms(4) have "False" 
+      by simp
+    then show ?thesis by simp
+  next
+    case new_pending
+    with assms have "length t = length l " "length (t ! rep_of l a\<^sub>1) = length l" 
+       apply simp using assms rep_of_less_length_l unfolding lookup_invar_def 
+      by fastforce
+    with assms(5) have "lookup_entry (update_lookup t l u1) l a\<^sub>1 a\<^sub>2 = Some u1" 
+      by (simp add: assms(3) assms(6) assms(7) rep_of_less_length_l)
+    with assms have "(F (rep_of l a\<^sub>1) (rep_of l a\<^sub>2) \<approx> rep_of l a) \<in> representativeE
        \<lparr>cc_list = l, use_list = u[rep_b := u1 # u ! rep_b], lookup = update_lookup t l u1,
           pending = pe, proof_forest = pf, pf_labels = pfl, input = ip\<rparr>"
-        unfolding representativeE_def congruence_closure.select_convs 
-        using rep_of_less_length_l rep_of_min by fastforce
-      then show ?thesis using CC_F_rep_of_a_imp_F_a base 
-        by (simp add: Congruence_Closure_union assms(5) assms(6) assms(7) assms(8) new_pending)      
-    qed (simp_all add: base representativeE_def)
+      unfolding representativeE_def congruence_closure.select_convs 
+      using rep_of_less_length_l rep_of_min by fastforce
+    then show ?thesis using CC_F_rep_of_a_imp_F_a base 
+      by (simp add: Congruence_Closure_union assms(5) assms(6) assms(7) assms(8) new_pending)      
+  qed (simp_all add: base representativeE_def)
+qed
+
+
+lemma in_set_Cons_use_list:
+  assumes "rep_b' < length u" 
+"i \<noteq> rep_of l a " "eq \<in> set (u ! i) "
+  shows "i \<noteq> rep_of l a
+\<Longrightarrow> eq \<in> set (u ! i) \<Longrightarrow> eq \<in> set ((u[rep_b' := u1' # u ! rep_b']) ! i)"
+  proof(cases "i = rep_b'")
+    case True
+    from True have "u[rep_b' := u1' # u ! rep_b'] ! i = u1' # u ! rep_b'"
+      by (simp add: assms)
+    with True assms show ?thesis 
+      by force
+  next
+    case False
+  from False have "u[rep_b' := u1' # u ! rep_b'] ! i = u ! i"
+    by auto
+  then show ?thesis 
+    using assms by auto
+qed
+lemma lookup_invar2_loop1:
+  assumes "ufa_invar l" 
+    "a < length l" "b < length l" 
+    "use_list_invar
+\<lparr>cc_list = ufa_union l a b, use_list = u, lookup = t, pending = pe, proof_forest = pf, pf_labels = pfl, input = ip\<rparr>
+"
+    "lookup_invar
+\<lparr>cc_list = ufa_union l a b, use_list = u, lookup = t, pending = pe, proof_forest = pf, pf_labels = pfl, input = ip\<rparr>"
+
+"lookup_invar2'
+     \<lparr>cc_list = ufa_union l a b, use_list = u, lookup = t, pending = pe, proof_forest = pf,
+        pf_labels = pfl, input = ip\<rparr>
+     (u1' # urest')"
+(is "lookup_invar2' ?base (u1' # urest')")
+"rep_of l a \<noteq> rep_of l b"
+"lookup_Some t (ufa_union l a b) u1'"
+"u1' = (F d\<^sub>1 d\<^sub>2 \<approx> d)" "d\<^sub>1 < length l" "d\<^sub>2 < length l" 
+shows "lookup_invar2'
+     \<lparr>cc_list = ufa_union l a b, use_list = u, lookup = t,
+        pending = link_to_lookup t (ufa_union l a b) u1' # pe, proof_forest = pf,
+        pf_labels = pfl, input = ip\<rparr> urest'"
+  (is "lookup_invar2' ?loop1 urest'")
+  unfolding lookup_invar2'_def congruence_closure.select_convs
+proof(standard, standard, standard, standard, standard, standard, standard, standard, standard, standard)
+  have ufa_invar_mini_step: "ufa_invar (ufa_union l a b)" 
+    by (simp add: assms(1,2,3) ufa_union_invar)
+  have CC_loop1: "Congruence_Closure
+   (representativeE ?base \<union> pending_set pe \<union> set (u1' # urest'))
+= Congruence_Closure
+            (representativeE ?loop1 \<union>
+             pending_set (link_to_lookup t (ufa_union l a b) u1' # pe)
+\<union> set urest')" 
+    using inv2_loop1 assms 
+    by (metis length_list_update ufa_invar_mini_step)
+  fix a' b' c c\<^sub>1 c\<^sub>2
+  assume prems: "a' < length (ufa_union l a b)"
+    "b' < length (ufa_union l a b)"
+    "ufa_union l a b ! a' = a'"
+    "ufa_union l a b ! b' = b'"
+    "t ! a' ! b' = Some (F c\<^sub>1 c\<^sub>2 \<approx> c)" 
+  from prems have *: "l ! a' = a'" "l ! b' = b'" "a' < length l" "b' < length l" 
+    using assms(1-3) ufa_union_root apply blast+
+    using prems by auto
+  with prems assms have "a' \<noteq> rep_of l a" "b' \<noteq> rep_of l a" 
+    by (metis nth_list_update_eq)+
+  with assms * prems obtain b\<^sub>1 b\<^sub>2 cb a\<^sub>1 a\<^sub>2 ca where use_list: "F a\<^sub>1 a\<^sub>2 \<approx> ca \<in> set (u ! a') \<and>
+           rep_of (ufa_union l a b) a\<^sub>1 = rep_of (ufa_union l a b) c\<^sub>1 \<and>
+           rep_of (ufa_union l a b) a\<^sub>2 = rep_of (ufa_union l a b) c\<^sub>2 \<and>
+           Congruence_Closure
+            (representativeE
+              ?base \<union>
+             pending_set (pe) \<union>
+             set (u1' # urest'))
+            (ca \<approx> c) 
+       ""
+           F b\<^sub>1 b\<^sub>2 \<approx> cb \<in> set (u ! b') \<and>
+           rep_of (ufa_union l a b) b\<^sub>1 = rep_of (ufa_union l a b) c\<^sub>1 \<and>
+           rep_of (ufa_union l a b) b\<^sub>2 = rep_of (ufa_union l a b) c\<^sub>2 \<and>
+           Congruence_Closure
+            (representativeE
+              ?base \<union>
+             pending_set (pe) \<union>
+             set (u1' # urest'))
+            (cb \<approx> c)" unfolding lookup_invar2'_def congruence_closure.select_convs
+    by blast
+  with assms * use_list_invar_less_n_in_set use_list
+    prems * lookup_invar_less_n length_list_update
+  have length_b: "b\<^sub>1 < length l" "b\<^sub>2 < length l" "cb < length l" "a\<^sub>1 < length l" "a\<^sub>2 < length l" 
+    "ca < length l" "c\<^sub>1 < length l" "c\<^sub>2 < length l"
+    by metis+
+  with rep_of_ufa_union_invar assms(1,2,3) use_list
+  have "rep_of (ufa_union l a b) a\<^sub>1 = rep_of (ufa_union l a b) c\<^sub>1"
+    "rep_of (ufa_union l a b) a\<^sub>2 = rep_of (ufa_union l a b) c\<^sub>2"
+    " rep_of (ufa_union l a b) b\<^sub>1 = rep_of (ufa_union l a b) c\<^sub>1"
+    "rep_of (ufa_union l a b) b\<^sub>2 = rep_of (ufa_union l a b) c\<^sub>2"
+    by metis+
+  with use_list length_b have "(F a\<^sub>1 a\<^sub>2 \<approx> ca) \<in> set (u ! a') \<and>
+           rep_of (ufa_union l a b) a\<^sub>1 = rep_of (ufa_union l a b) c\<^sub>1 \<and>
+           rep_of (ufa_union l a b) a\<^sub>2 = rep_of (ufa_union l a b) c\<^sub>2 \<and>
+           Congruence_Closure
+            (representativeE
+              ?loop1 \<union>
+             pending_set (link_to_lookup t (ufa_union l a b) u1' # pe) \<union>
+      set urest')
+            (ca \<approx> c) 
+       ""
+           (F b\<^sub>1 b\<^sub>2 \<approx> cb) \<in> set (u ! b') \<and>
+           rep_of (ufa_union l a b) b\<^sub>1 = rep_of (ufa_union l a b) c\<^sub>1 \<and>
+           rep_of (ufa_union l a b) b\<^sub>2 = rep_of (ufa_union l a b) c\<^sub>2 \<and>
+           Congruence_Closure
+            (representativeE
+              ?loop1 \<union>
+             pending_set (link_to_lookup t (ufa_union l a b) u1' # pe) \<union>
+      set urest')
+            (cb \<approx> c)"
+    unfolding CC_loop1 
+    by blast+
+  then show "(\<exists>b\<^sub>1 b\<^sub>2 ba.
+           (F b\<^sub>1 b\<^sub>2 \<approx> ba) \<in> set (u ! a') \<and>
+           rep_of (ufa_union l a b) b\<^sub>1 = rep_of (ufa_union l a b) c\<^sub>1 \<and>
+           rep_of (ufa_union l a b) b\<^sub>2 = rep_of (ufa_union l a b) c\<^sub>2 \<and>
+           Congruence_Closure
+            (representativeE
+              \<lparr>cc_list = ufa_union l a b, use_list = u, lookup = t,
+                 pending = link_to_lookup t (ufa_union l a b) u1' # pe, proof_forest = pf,
+                 pf_labels = pfl, input = ip\<rparr> \<union>
+             pending_set (link_to_lookup t (ufa_union l a b) u1' # pe) \<union>
+             set urest')
+            (ba \<approx> c)) \<and>
+       (\<exists>b\<^sub>1 b\<^sub>2 ba.
+           (F b\<^sub>1 b\<^sub>2 \<approx> ba) \<in> set (u ! b') \<and>
+           rep_of (ufa_union l a b) b\<^sub>1 = rep_of (ufa_union l a b) c\<^sub>1 \<and>
+           rep_of (ufa_union l a b) b\<^sub>2 = rep_of (ufa_union l a b) c\<^sub>2 \<and>
+           Congruence_Closure
+            (representativeE
+              \<lparr>cc_list = ufa_union l a b, use_list = u, lookup = t,
+                 pending = link_to_lookup t (ufa_union l a b) u1' # pe, proof_forest = pf,
+                 pf_labels = pfl, input = ip\<rparr> \<union>
+             pending_set (link_to_lookup t (ufa_union l a b) u1' # pe) \<union>
+             set urest')
+            (ba \<approx> c))"
+    using assms by auto
+qed
+
+lemma lookup_invar2_loop2:
+  assumes "ufa_invar l" 
+    "a < length l" "b < length l" 
+    "use_list_invar
+\<lparr>cc_list = ufa_union l a b, use_list = u, lookup = t, pending = pe, proof_forest = pf, pf_labels = pfl, input = ip\<rparr>
+"
+    "lookup_invar
+\<lparr>cc_list = ufa_union l a b, use_list = u, lookup = t, pending = pe, proof_forest = pf, pf_labels = pfl, input = ip\<rparr>"
+
+"lookup_invar2'
+     \<lparr>cc_list = ufa_union l a b, use_list = u, lookup = t, pending = pe, proof_forest = pf,
+        pf_labels = pfl, input = ip\<rparr>
+     (u1' # urest')"
+(is "lookup_invar2' ?base (u1' # urest')")
+"rep_of l a \<noteq> rep_of l b"
+"\<not> lookup_Some t (ufa_union l a b) u1'"
+"u1' = (F d\<^sub>1 d\<^sub>2 \<approx> d)" "d\<^sub>1 < length l" "d\<^sub>2 < length l"  "d < length l"
+
+"length l = length t"
+"rep_b' < length u"
+ "(rep_of l d\<^sub>1 \<noteq> rep_of l a \<longrightarrow> 
+contains_similar_equation \<lparr>cc_list = ufa_union l a b, 
+    use_list = u, 
+    lookup = t, 
+    pending = pe,
+    proof_forest = pf, 
+    pf_labels = pfl, 
+    input = ip\<rparr> (rep_of l d\<^sub>1) d\<^sub>1 d\<^sub>2 d (u1' # urest'))
+
+\<and> 
+(rep_of l d\<^sub>2 \<noteq> rep_of l a \<longrightarrow> 
+contains_similar_equation \<lparr>cc_list = ufa_union l a b, 
+    use_list = u, 
+    lookup = t, 
+    pending = pe,
+    proof_forest = pf, 
+    pf_labels = pfl, 
+    input = ip\<rparr> (rep_of l d\<^sub>2) d\<^sub>1 d\<^sub>2 d (u1' # urest'))
+"
+"rep_of l a = rep_of l d\<^sub>1 \<or> rep_of l a = rep_of l d\<^sub>2"
+"rep_b' = rep_of l b"
+shows "lookup_invar2'
+     \<lparr>cc_list = ufa_union l a b, use_list = u[rep_b' := u1' # u ! rep_b'], 
+lookup = update_lookup t (ufa_union l a b) u1', 
+pending = pe, proof_forest = pf,
+       pf_labels = pfl, input = ip\<rparr> urest'"
+(is "lookup_invar2' ?loop2 urest'")
+  unfolding lookup_invar2'_def congruence_closure.select_convs
+proof(standard, standard, standard, standard, standard, standard, standard, standard, standard, standard)
+  have ufa_invar_mini_step: "ufa_invar (ufa_union l a b)" 
+    by (simp add: assms(1,2,3) ufa_union_invar)
+  have CC_loop2: "Congruence_Closure
+   (representativeE ?base \<union> pending_set pe \<union> set (u1' # urest'))
+= Congruence_Closure
+            (representativeE ?loop2 \<union>
+             pending_set pe
+\<union> set urest')" 
+    using inv2_loop2 assms 
+    by (metis length_list_update ufa_invar_mini_step)
+  fix a' b' c c\<^sub>1 c\<^sub>2
+  assume prems: "a' < length (ufa_union l a b)"
+    "b' < length (ufa_union l a b)"
+    "ufa_union l a b ! a' = a'"
+    "ufa_union l a b ! b' = b'"
+    "update_lookup t (ufa_union l a b) u1' ! a' ! b' = Some (F c\<^sub>1 c\<^sub>2 \<approx> c)" 
+  from prems have *: "l ! a' = a'" "l ! b' = b'" "a' < length l" "b' < length l" 
+    using assms(1-3) ufa_union_root apply blast+
+    using prems by auto
+  with prems assms have "a' \<noteq> rep_of l a" "b' \<noteq> rep_of l a" 
+    by (metis nth_list_update_eq)+
+  have "update_lookup t (ufa_union l a b) u1' ! a' ! b' \<noteq> None" 
+    using prems by fast
+  with assms(5) prems obtain k\<^sub>1 k\<^sub>2 k where 
+"update_lookup t (ufa_union l a b) u1' ! a' ! b' = Some (F k\<^sub>1 k\<^sub>2 \<approx> k)" 
+     "rep_of (ufa_union l a b) k\<^sub>1 = a'" "rep_of (ufa_union l a b) k\<^sub>2 = b'"
+    unfolding lookup_invar_def congruence_closure.select_convs     
+    by (smt (verit, ccfv_threshold) "*"(3,4) assms(13,9) nth_list_update_eq update_lookup.simps(1) update_lookup_unchanged)
+  then have a_b: "rep_of (ufa_union l a b) c\<^sub>1 = a'" "rep_of (ufa_union l a b) c\<^sub>2 = b'"
+    using prems(5) by auto
+  show "(\<exists>b\<^sub>1 b\<^sub>2 ba.
+           (F b\<^sub>1 b\<^sub>2 \<approx> ba) \<in> set (u[rep_b' := u1' # u ! rep_b'] ! a') \<and>
+           rep_of (ufa_union l a b) b\<^sub>1 = rep_of (ufa_union l a b) c\<^sub>1 \<and>
+           rep_of (ufa_union l a b) b\<^sub>2 = rep_of (ufa_union l a b) c\<^sub>2 \<and>
+           Congruence_Closure
+            (representativeE
+              \<lparr>cc_list = ufa_union l a b, use_list = u[rep_b' := u1' # u ! rep_b'],
+                 lookup = update_lookup t (ufa_union l a b) u1', pending = pe, proof_forest = pf,
+                 pf_labels = pfl, input = ip\<rparr> \<union>
+             pending_set pe \<union>
+             set urest')
+            (ba \<approx> c)) \<and>
+       (\<exists>b\<^sub>1 b\<^sub>2 ba.
+           (F b\<^sub>1 b\<^sub>2 \<approx> ba) \<in> set (u[rep_b' := u1' # u ! rep_b'] ! b') \<and>
+           rep_of (ufa_union l a b) b\<^sub>1 = rep_of (ufa_union l a b) c\<^sub>1 \<and>
+           rep_of (ufa_union l a b) b\<^sub>2 = rep_of (ufa_union l a b) c\<^sub>2 \<and>
+           Congruence_Closure
+            (representativeE
+              \<lparr>cc_list = ufa_union l a b, use_list = u[rep_b' := u1' # u ! rep_b'],
+                 lookup = update_lookup t (ufa_union l a b) u1', pending = pe, proof_forest = pf,
+                 pf_labels = pfl, input = ip\<rparr> \<union>
+             pending_set pe \<union>
+             set urest')
+            (ba \<approx> c))"
+proof(cases "update_lookup t (ufa_union l a b) u1' ! a' ! b' = t ! a' ! b'")
+  case True
+  with assms * prems obtain b\<^sub>1 b\<^sub>2 cb a\<^sub>1 a\<^sub>2 ca where use_list: "F a\<^sub>1 a\<^sub>2 \<approx> ca \<in> set (u ! a') \<and>
+           rep_of (ufa_union l a b) a\<^sub>1 = rep_of (ufa_union l a b) c\<^sub>1 \<and>
+           rep_of (ufa_union l a b) a\<^sub>2 = rep_of (ufa_union l a b) c\<^sub>2 \<and>
+           Congruence_Closure
+            (representativeE
+              ?base \<union>
+             pending_set (pe) \<union>
+             set (u1' # urest'))
+            (ca \<approx> c) 
+       ""
+           F b\<^sub>1 b\<^sub>2 \<approx> cb \<in> set (u ! b') \<and>
+           rep_of (ufa_union l a b) b\<^sub>1 = rep_of (ufa_union l a b) c\<^sub>1 \<and>
+           rep_of (ufa_union l a b) b\<^sub>2 = rep_of (ufa_union l a b) c\<^sub>2 \<and>
+           Congruence_Closure
+            (representativeE
+              ?base \<union>
+             pending_set pe \<union>
+             set (u1' # urest'))
+            (cb \<approx> c)" unfolding lookup_invar2'_def congruence_closure.select_convs True
+    by blast
+  with assms * use_list_invar_less_n_in_set use_list
+    prems True * lookup_invar_less_n length_list_update
+  have length_b: "b\<^sub>1 < length l" "b\<^sub>2 < length l" "cb < length l" "a\<^sub>1 < length l" "a\<^sub>2 < length l" 
+    "ca < length l" "c\<^sub>1 < length l" "c\<^sub>2 < length l"
+    by metis+
+  with rep_of_ufa_union_invar assms(1,2,3) use_list
+  have "rep_of (ufa_union l a b) a\<^sub>1 = rep_of (ufa_union l a b) c\<^sub>1"
+    "rep_of (ufa_union l a b) a\<^sub>2 = rep_of (ufa_union l a b) c\<^sub>2"
+    " rep_of (ufa_union l a b) b\<^sub>1 = rep_of (ufa_union l a b) c\<^sub>1"
+    "rep_of (ufa_union l a b) b\<^sub>2 = rep_of (ufa_union l a b) c\<^sub>2"
+    by metis+
+  with use_list length_b have *: "(F a\<^sub>1 a\<^sub>2 \<approx> ca) \<in> set (u ! a') \<and>
+           rep_of (ufa_union l a b) a\<^sub>1 = rep_of (ufa_union l a b) c\<^sub>1 \<and>
+           rep_of (ufa_union l a b) a\<^sub>2 = rep_of (ufa_union l a b) c\<^sub>2 \<and>
+           Congruence_Closure
+            (representativeE
+              ?loop2 \<union>
+             pending_set pe \<union>
+      set urest')
+            (ca \<approx> c) 
+       ""
+           (F b\<^sub>1 b\<^sub>2 \<approx> cb) \<in> set (u ! b') \<and>
+           rep_of (ufa_union l a b) b\<^sub>1 = rep_of (ufa_union l a b) c\<^sub>1 \<and>
+           rep_of (ufa_union l a b) b\<^sub>2 = rep_of (ufa_union l a b) c\<^sub>2 \<and>
+           Congruence_Closure
+            (representativeE
+              ?loop2 \<union>
+             pending_set pe \<union>
+      set urest')
+            (cb \<approx> c)"
+    unfolding CC_loop2
+    by blast+
+  have "i \<noteq> rep_of l a 
+\<Longrightarrow> eq \<in> set (u ! i) \<Longrightarrow> eq \<in> set ((u[rep_b' := u1' # u ! rep_b']) ! i)"
+    for eq i using assms(14) in_set_Cons_use_list 
+    by fast 
+  with * show ?thesis
+    using \<open>a' \<noteq> rep_of l a\<close> \<open>b' \<noteq> rep_of l a\<close> by blast
+next
+  case False
+  with prems(5) have u1': "u1' = (F c\<^sub>1 c\<^sub>2 \<approx> c)" 
+    unfolding assms(9) update_lookup.simps by (metis nth_list_update' option.inject)
+  have u1_in_set: "F c\<^sub>1 c\<^sub>2 \<approx> c \<in> set (u[rep_b' := u1' # u ! rep_b'] ! rep_of l b)" 
+    using assms(14) u1' assms(17) assms(9) assms(17) by auto
+  have eq_rep_l_b: "eq \<in> set (u ! rep_of l b)
+\<Longrightarrow> eq \<in> set (u[rep_b' := u1' # u ! rep_b'] ! rep_of l b)" for eq 
+    by (metis assms(14) assms(7) in_set_Cons_use_list)
+have eq_not_rep_l_b: "rep_of l b \<noteq> kk \<Longrightarrow> eq \<in> set (u ! kk)
+\<Longrightarrow> eq \<in> set (u[rep_b' := u1' # u ! rep_b'] ! kk)" for eq kk
+    by (metis assms(14) assms(7) in_set_Cons_use_list)
+  consider "rep_of l a = rep_of l c\<^sub>1" "rep_of l a \<noteq> rep_of l c\<^sub>2"
+    | "rep_of l a = rep_of l c\<^sub>1" "rep_of l a = rep_of l c\<^sub>2"
+    | "rep_of l a \<noteq> rep_of l c\<^sub>1" "rep_of l a = rep_of l c\<^sub>2"
+    using \<open>u1' = F c\<^sub>1 c\<^sub>2 \<approx> c\<close> assms(16) assms(9) by fastforce
+  then show ?thesis proof(cases)
+    case 1
+    with a_b have "a' = rep_of l b"
+      using \<open>u1' = F c\<^sub>1 c\<^sub>2 \<approx> c\<close> assms ufa_union_aux by simp
+    have "(\<exists>b\<^sub>1 b\<^sub>2 ba.
+        (F b\<^sub>1 b\<^sub>2 \<approx> ba) \<in> set (u[rep_b' := u1' # u ! rep_b'] ! a') \<and>
+        rep_of (ufa_union l a b) b\<^sub>1 = rep_of (ufa_union l a b) c\<^sub>1 \<and>
+        rep_of (ufa_union l a b) b\<^sub>2 = rep_of (ufa_union l a b) c\<^sub>2 \<and>
+        Congruence_Closure
+         (representativeE
+           \<lparr>cc_list = ufa_union l a b, use_list = u[rep_b' := u1' # u ! rep_b'],
+              lookup = update_lookup t (ufa_union l a b) u1', pending = pe, proof_forest = pf,
+              pf_labels = pfl, input = ip\<rparr> \<union>
+          pending_set pe \<union>
+          set urest')
+         (ba \<approx> c))" 
+      by (smt (verit) "1"(2) CC_loop2 Congruence_Closure.symmetric \<open>a' = rep_of l b\<close> assms(15) assms(9) congruence_closure.select_convs(4) equation.inject(2) transitive1 u1' u1_in_set)
+    then show ?thesis 
+      by (smt (z3) CC_loop2 \<open>a' = rep_of l b\<close> a_b assms(1) assms(11) assms(15) assms(2) assms(3) assms(9) congruence_closure.select_convs(1) congruence_closure.select_convs(2) congruence_closure.select_convs(4) eq_not_rep_l_b equation.inject(2) option.inject prems(5) u1' ufa_union_aux)
+  next
+    case 2
+    then show ?thesis 
+      by (metis Congruence_Closure.reflexive a_b(1) a_b(2) assms(1) assms(10) assms(11) assms(3) assms(9) equation.inject(2) u1' u1_in_set ufa_union_aux)
+  next
+    case 3
+    then show ?thesis 
+      by (smt (verit, best) CC_loop2 Congruence_Closure.reflexive \<open>rep_of (ufa_union l a b) k\<^sub>1 = a'\<close> \<open>rep_of (ufa_union l a b) k\<^sub>2 = b'\<close> \<open>update_lookup t (ufa_union l a b) u1' ! a' ! b' = Some (F k\<^sub>1 k\<^sub>2 \<approx> k)\<close> assms(1) assms(10) assms(11) assms(15) assms(3) assms(9) congruence_closure.select_convs(1) congruence_closure.select_convs(2) congruence_closure.select_convs(4) eq_not_rep_l_b equation.inject(2) option.inject prems(5) u1' u1_in_set ufa_union_aux)
   qed
+qed
+qed
+
+lemma lookup_invar2_prems_loop1:
+  assumes "\<forall>eq'\<in>set (u1' # urest').
+       \<exists>c\<^sub>1 c\<^sub>2 c.
+          eq' = F c\<^sub>1 c\<^sub>2 \<approx> c \<and>
+          c\<^sub>1 < length l \<and>
+          c\<^sub>2 < length l \<and>
+          c < length l \<and>
+          (rep_of l c\<^sub>1 \<noteq> rep_of l a \<longrightarrow>
+           contains_similar_equation
+            \<lparr>cc_list = ufa_union l a b, use_list = u, lookup = t, pending = pe, proof_forest = pf,
+               pf_labels = pfl, input = ip\<rparr>
+            (rep_of l c\<^sub>1) c\<^sub>1 c\<^sub>2 c (u1' # urest')) \<and>
+          (rep_of l c\<^sub>2 \<noteq> rep_of l a \<longrightarrow>
+           contains_similar_equation
+            \<lparr>cc_list = ufa_union l a b, use_list = u, lookup = t, pending = pe, proof_forest = pf,
+               pf_labels = pfl, input = ip\<rparr>
+            (rep_of l c\<^sub>2) c\<^sub>1 c\<^sub>2 c (u1' # urest'))"
+"lookup_invar \<lparr>cc_list = ufa_union l a b, use_list = u, lookup = t, pending = pe, proof_forest = pf,
+               pf_labels = pfl, input = ip\<rparr>"
+"ufa_invar (ufa_union l a b)" "lookup_Some t (ufa_union l a b) u1'"
+"u1' = (F a\<^sub>1 a\<^sub>2 \<approx> aa)" "a\<^sub>1 < length (ufa_union l a b)" "a\<^sub>2 < length (ufa_union l a b)"
+  shows "\<forall>eq'\<in>set urest'.
+       \<exists>c\<^sub>1 c\<^sub>2 c.
+          eq' = F c\<^sub>1 c\<^sub>2 \<approx> c \<and>
+          c\<^sub>1 < length l \<and>
+          c\<^sub>2 < length l \<and>
+          c < length l \<and>
+          (rep_of l c\<^sub>1 \<noteq> rep_of l a \<longrightarrow>
+           contains_similar_equation
+            \<lparr>cc_list = ufa_union l a b, use_list = u, lookup = t,
+               pending = link_to_lookup t (ufa_union l a b) u1' # pe, proof_forest = pf, pf_labels = pfl,
+               input = ip\<rparr>
+            (rep_of l c\<^sub>1) c\<^sub>1 c\<^sub>2 c urest') \<and>
+          (rep_of l c\<^sub>2 \<noteq> rep_of l a \<longrightarrow>
+           contains_similar_equation
+            \<lparr>cc_list = ufa_union l a b, use_list = u, lookup = t,
+               pending = link_to_lookup t (ufa_union l a b) u1' # pe, proof_forest = pf, pf_labels = pfl,
+               input = ip\<rparr>
+            (rep_of l c\<^sub>2) c\<^sub>1 c\<^sub>2 c urest')"
+proof
+  fix eq'
+  assume "eq' \<in> set urest'"
+  then have "eq' \<in> set (u1' # urest')"
+    by fastforce
+  with assms obtain c\<^sub>1 c\<^sub>2 c where *: "eq' = (F c\<^sub>1 c\<^sub>2 \<approx> c) \<and>
+          c\<^sub>1 < length l \<and>
+          c\<^sub>2 < length l \<and>
+          c < length l \<and>
+          (rep_of l c\<^sub>1 \<noteq> rep_of l a \<longrightarrow>
+           (\<exists>b\<^sub>1 b\<^sub>2 ba.
+               (F b\<^sub>1 b\<^sub>2 \<approx> ba) \<in> set (u ! rep_of l c\<^sub>1) \<and>
+               rep_of (ufa_union l a b) b\<^sub>1 = rep_of (ufa_union l a b) c\<^sub>1 \<and>
+               rep_of (ufa_union l a b) b\<^sub>2 = rep_of (ufa_union l a b) c\<^sub>2 \<and>
+               Congruence_Closure
+                (representativeE
+                  \<lparr>cc_list = ufa_union l a b, use_list = u, lookup = t, pending = pe,
+                     proof_forest = pf, pf_labels = pfl, input = ip\<rparr> \<union>
+                 pending_set pe \<union>
+                 set (u1' # urest'))
+                (ba \<approx> c))) \<and>
+          (rep_of l c\<^sub>2 \<noteq> rep_of l a \<longrightarrow>
+           (\<exists>b\<^sub>1 b\<^sub>2 ba.
+               (F b\<^sub>1 b\<^sub>2 \<approx> ba) \<in> set (u ! rep_of l c\<^sub>2) \<and>
+               rep_of (ufa_union l a b) b\<^sub>1 = rep_of (ufa_union l a b) c\<^sub>1 \<and>
+               rep_of (ufa_union l a b) b\<^sub>2 = rep_of (ufa_union l a b) c\<^sub>2 \<and>
+               Congruence_Closure
+                (representativeE
+                  \<lparr>cc_list = ufa_union l a b, use_list = u, lookup = t, pending = pe,
+                     proof_forest = pf, pf_labels = pfl, input = ip\<rparr> \<union>
+                 pending_set pe \<union>
+                 set (u1' # urest'))
+                (ba \<approx> c)))" unfolding congruence_closure.select_convs
+    by fast
+  from inv2_loop1[OF assms(2,3,4,5,6,7)] have "Congruence_Closure
+                (representativeE
+                  \<lparr>cc_list = ufa_union l a b, use_list = u, lookup = t, pending = pe,
+                     proof_forest = pf, pf_labels = pfl, input = ip\<rparr> \<union>
+                 pending_set pe \<union>
+                 set (u1' # urest')) = Congruence_Closure
+                    (representativeE
+                      \<lparr>cc_list = ufa_union l a b, use_list = u, lookup = t,
+                         pending = link_to_lookup t (ufa_union l a b) u1' # pe, proof_forest = pf,
+                         pf_labels = pfl, input = ip\<rparr> \<union>
+                     pending_set (link_to_lookup t (ufa_union l a b) u1' # pe) \<union>
+                     set urest')"
+    by simp
+  then have "eq' = (F c\<^sub>1 c\<^sub>2 \<approx> c) \<and>
+              c\<^sub>1 < length l \<and>
+              c\<^sub>2 < length l \<and>
+              c < length l \<and>
+              (rep_of l c\<^sub>1 \<noteq> rep_of l a \<longrightarrow>
+               (\<exists>b\<^sub>1 b\<^sub>2 ba.
+                   (F b\<^sub>1 b\<^sub>2 \<approx> ba) \<in> set (u ! rep_of l c\<^sub>1) \<and>
+                   rep_of (ufa_union l a b) b\<^sub>1 = rep_of (ufa_union l a b) c\<^sub>1 \<and>
+                   rep_of (ufa_union l a b) b\<^sub>2 = rep_of (ufa_union l a b) c\<^sub>2 \<and>
+                   Congruence_Closure
+                    (representativeE
+                      \<lparr>cc_list = ufa_union l a b, use_list = u, lookup = t,
+                         pending = link_to_lookup t (ufa_union l a b) u1' # pe, proof_forest = pf,
+                         pf_labels = pfl, input = ip\<rparr> \<union>
+                     pending_set (link_to_lookup t (ufa_union l a b) u1' # pe) \<union>
+                     set urest')
+                    (ba \<approx> c))) \<and>
+              (rep_of l c\<^sub>2 \<noteq> rep_of l a \<longrightarrow>
+               (\<exists>b\<^sub>1 b\<^sub>2 ba.
+                   (F b\<^sub>1 b\<^sub>2 \<approx> ba) \<in> set (u ! rep_of l c\<^sub>2) \<and>
+                   rep_of (ufa_union l a b) b\<^sub>1 = rep_of (ufa_union l a b) c\<^sub>1 \<and>
+                   rep_of (ufa_union l a b) b\<^sub>2 = rep_of (ufa_union l a b) c\<^sub>2 \<and>
+                   Congruence_Closure
+                    (representativeE
+                      \<lparr>cc_list = ufa_union l a b, use_list = u, lookup = t,
+                         pending = link_to_lookup t (ufa_union l a b) u1' # pe, proof_forest = pf,
+                         pf_labels = pfl, input = ip\<rparr> \<union>
+                     pending_set (link_to_lookup t (ufa_union l a b) u1' # pe) \<union>
+                     set urest')
+                    (ba \<approx> c)))"
+    using "*" by presburger
+  then show "\<exists>c\<^sub>1 c\<^sub>2 c.
+              eq' = F c\<^sub>1 c\<^sub>2 \<approx> c \<and>
+              c\<^sub>1 < length l \<and>
+              c\<^sub>2 < length l \<and>
+              c < length l \<and>
+              (rep_of l c\<^sub>1 \<noteq> rep_of l a \<longrightarrow>
+               contains_similar_equation
+                \<lparr>cc_list = ufa_union l a b, use_list = u, lookup = t,
+                   pending = link_to_lookup t (ufa_union l a b) u1' # pe, proof_forest = pf, pf_labels = pfl,
+                   input = ip\<rparr>
+                (rep_of l c\<^sub>1) c\<^sub>1 c\<^sub>2 c urest') \<and>
+              (rep_of l c\<^sub>2 \<noteq> rep_of l a \<longrightarrow>
+               contains_similar_equation
+                \<lparr>cc_list = ufa_union l a b, use_list = u, lookup = t,
+                   pending = link_to_lookup t (ufa_union l a b) u1' # pe, proof_forest = pf, pf_labels = pfl,
+                   input = ip\<rparr>
+                (rep_of l c\<^sub>2) c\<^sub>1 c\<^sub>2 c urest')" 
+    unfolding congruence_closure.select_convs by blast
+qed
+
+
+lemma lookup_invar2_prems_loop2:
+  assumes "\<forall>eq'\<in>set (u1' # urest').
+       \<exists>c\<^sub>1 c\<^sub>2 c.
+          eq' = F c\<^sub>1 c\<^sub>2 \<approx> c \<and>
+          c\<^sub>1 < length l \<and>
+          c\<^sub>2 < length l \<and>
+          c < length l \<and>
+          (rep_of l c\<^sub>1 \<noteq> rep_of l a \<longrightarrow>
+           contains_similar_equation
+            \<lparr>cc_list = ufa_union l a b, use_list = u, lookup = t, pending = pe, proof_forest = pf,
+               pf_labels = pfl, input = ip\<rparr>
+            (rep_of l c\<^sub>1) c\<^sub>1 c\<^sub>2 c (u1' # urest')) \<and>
+          (rep_of l c\<^sub>2 \<noteq> rep_of l a \<longrightarrow>
+           contains_similar_equation
+            \<lparr>cc_list = ufa_union l a b, use_list = u, lookup = t, pending = pe, proof_forest = pf,
+               pf_labels = pfl, input = ip\<rparr>
+            (rep_of l c\<^sub>2) c\<^sub>1 c\<^sub>2 c (u1' # urest'))"
+
+"lookup_invar \<lparr>cc_list = ufa_union l a b, use_list = u, lookup = t, pending = pe, proof_forest = pf,
+               pf_labels = pfl, input = ip\<rparr>"
+"length (ufa_union l a b) = length t"
+"ufa_invar (ufa_union l a b)" 
+ "\<not> lookup_Some t (ufa_union l a b) u1'"
+"u1' = (F a\<^sub>1 a\<^sub>2 \<approx> aa)" "a\<^sub>1 < length (ufa_union l a b)" "a\<^sub>2 < length (ufa_union l a b)"
+"aa < length (ufa_union l a b)"
+"rep_b' < length u"
+  shows "\<forall>eq'\<in>set urest'.
+       \<exists>c\<^sub>1 c\<^sub>2 c.
+          eq' = F c\<^sub>1 c\<^sub>2 \<approx> c \<and>
+          c\<^sub>1 < length l \<and>
+          c\<^sub>2 < length l \<and>
+          c < length l \<and>
+          (rep_of l c\<^sub>1 \<noteq> rep_of l a \<longrightarrow>
+           contains_similar_equation
+            \<lparr>cc_list = ufa_union l a b, use_list = u[rep_b' := u1' # u ! rep_b'], 
+lookup = update_lookup t (ufa_union l a b) u1', 
+pending = pe, proof_forest = pf,
+       pf_labels = pfl, input = ip\<rparr>
+            (rep_of l c\<^sub>1) c\<^sub>1 c\<^sub>2 c urest') \<and>
+          (rep_of l c\<^sub>2 \<noteq> rep_of l a \<longrightarrow>
+           contains_similar_equation
+            \<lparr>cc_list = ufa_union l a b, use_list = u[rep_b' := u1' # u ! rep_b'], 
+lookup = update_lookup t (ufa_union l a b) u1', 
+pending = pe, proof_forest = pf,
+       pf_labels = pfl, input = ip\<rparr>
+            (rep_of l c\<^sub>2) c\<^sub>1 c\<^sub>2 c urest')"
+proof
+  fix eq'
+  assume "eq' \<in> set urest'"
+  then have "eq' \<in> set (u1' # urest')"
+    by fastforce
+  with assms obtain c\<^sub>1 c\<^sub>2 c where *: "eq' = (F c\<^sub>1 c\<^sub>2 \<approx> c) \<and>
+          c\<^sub>1 < length l \<and>
+          c\<^sub>2 < length l \<and>
+          c < length l \<and>
+          (rep_of l c\<^sub>1 \<noteq> rep_of l a \<longrightarrow>
+           (\<exists>b\<^sub>1 b\<^sub>2 ba.
+               (F b\<^sub>1 b\<^sub>2 \<approx> ba) \<in> set (u ! rep_of l c\<^sub>1) \<and>
+               rep_of (ufa_union l a b) b\<^sub>1 = rep_of (ufa_union l a b) c\<^sub>1 \<and>
+               rep_of (ufa_union l a b) b\<^sub>2 = rep_of (ufa_union l a b) c\<^sub>2 \<and>
+               Congruence_Closure
+                (representativeE
+                  \<lparr>cc_list = ufa_union l a b, use_list = u, lookup = t, pending = pe,
+                     proof_forest = pf, pf_labels = pfl, input = ip\<rparr> \<union>
+                 pending_set pe \<union>
+                 set (u1' # urest'))
+                (ba \<approx> c))) \<and>
+          (rep_of l c\<^sub>2 \<noteq> rep_of l a \<longrightarrow>
+           (\<exists>b\<^sub>1 b\<^sub>2 ba.
+               (F b\<^sub>1 b\<^sub>2 \<approx> ba) \<in> set (u ! rep_of l c\<^sub>2) \<and>
+               rep_of (ufa_union l a b) b\<^sub>1 = rep_of (ufa_union l a b) c\<^sub>1 \<and>
+               rep_of (ufa_union l a b) b\<^sub>2 = rep_of (ufa_union l a b) c\<^sub>2 \<and>
+               Congruence_Closure
+                (representativeE
+                  \<lparr>cc_list = ufa_union l a b, use_list = u, lookup = t, pending = pe,
+                     proof_forest = pf, pf_labels = pfl, input = ip\<rparr> \<union>
+                 pending_set pe \<union>
+                 set (u1' # urest'))
+                (ba \<approx> c)))" unfolding congruence_closure.select_convs
+    by fast
+  from inv2_loop2[OF assms(2,3,4,5,6,7,8,9)] have CC_step: "Congruence_Closure
+                (representativeE
+                  \<lparr>cc_list = ufa_union l a b, use_list = u, lookup = t, pending = pe,
+                     proof_forest = pf, pf_labels = pfl, input = ip\<rparr> \<union>
+                 pending_set pe \<union>
+                 set (u1' # urest')) = Congruence_Closure
+                    (representativeE
+                      \<lparr>cc_list = ufa_union l a b, use_list = u[rep_b' := u1' # u ! rep_b'], 
+lookup = update_lookup t (ufa_union l a b) u1', 
+pending = pe, proof_forest = pf,
+       pf_labels = pfl, input = ip\<rparr> \<union>
+                     pending_set pe \<union>
+                     set urest')"
+    by simp
+  have "i \<noteq> rep_of l a 
+\<Longrightarrow> eq \<in> set (u ! i) \<Longrightarrow> eq \<in> set ((u[rep_b' := u1' # u ! rep_b']) ! i)"
+    for eq i 
+    using assms(10) in_set_Cons_use_list by fast
+  then have "eq' = (F c\<^sub>1 c\<^sub>2 \<approx> c) \<and>
+              c\<^sub>1 < length l \<and>
+              c\<^sub>2 < length l \<and>
+              c < length l \<and>
+              (rep_of l c\<^sub>1 \<noteq> rep_of l a \<longrightarrow>
+               (\<exists>b\<^sub>1 b\<^sub>2 ba.
+                   (F b\<^sub>1 b\<^sub>2 \<approx> ba) \<in> set ((u[rep_b' := u1' # u ! rep_b']) ! rep_of l c\<^sub>1) \<and>
+                   rep_of (ufa_union l a b) b\<^sub>1 = rep_of (ufa_union l a b) c\<^sub>1 \<and>
+                   rep_of (ufa_union l a b) b\<^sub>2 = rep_of (ufa_union l a b) c\<^sub>2 \<and>
+                   Congruence_Closure
+                    (representativeE
+                      \<lparr>cc_list = ufa_union l a b, use_list = u[rep_b' := u1' # u ! rep_b'], 
+lookup = update_lookup t (ufa_union l a b) u1', 
+pending = pe, proof_forest = pf,
+       pf_labels = pfl, input = ip\<rparr> \<union>
+                     pending_set pe \<union>
+                     set urest')
+                    (ba \<approx> c))) \<and>
+              (rep_of l c\<^sub>2 \<noteq> rep_of l a \<longrightarrow>
+               (\<exists>b\<^sub>1 b\<^sub>2 ba.
+                   (F b\<^sub>1 b\<^sub>2 \<approx> ba) \<in> set ((u[rep_b' := u1' # u ! rep_b']) ! rep_of l c\<^sub>2) \<and>
+                   rep_of (ufa_union l a b) b\<^sub>1 = rep_of (ufa_union l a b) c\<^sub>1 \<and>
+                   rep_of (ufa_union l a b) b\<^sub>2 = rep_of (ufa_union l a b) c\<^sub>2 \<and>
+                    Congruence_Closure
+                    (representativeE
+                      \<lparr>cc_list = ufa_union l a b, use_list = u[rep_b' := u1' # u ! rep_b'], 
+lookup = update_lookup t (ufa_union l a b) u1', 
+pending = pe, proof_forest = pf,
+       pf_labels = pfl, input = ip\<rparr> \<union>
+                     pending_set pe \<union>
+                     set urest')
+                    (ba \<approx> c)))"
+    using "*" CC_step 
+    by metis
+  then show "\<exists>c\<^sub>1 c\<^sub>2 c.
+              eq' = F c\<^sub>1 c\<^sub>2 \<approx> c \<and>
+              c\<^sub>1 < length l \<and>
+              c\<^sub>2 < length l \<and>
+              c < length l \<and>
+              (rep_of l c\<^sub>1 \<noteq> rep_of l a \<longrightarrow>
+               contains_similar_equation
+                \<lparr>cc_list = ufa_union l a b, use_list = u[rep_b' := u1' # u ! rep_b'], 
+lookup = update_lookup t (ufa_union l a b) u1', 
+pending = pe, proof_forest = pf,
+       pf_labels = pfl, input = ip\<rparr>
+                (rep_of l c\<^sub>1) c\<^sub>1 c\<^sub>2 c urest') \<and>
+              (rep_of l c\<^sub>2 \<noteq> rep_of l a \<longrightarrow>
+               contains_similar_equation
+                \<lparr>cc_list = ufa_union l a b, use_list = u[rep_b' := u1' # u ! rep_b'], 
+lookup = update_lookup t (ufa_union l a b) u1', 
+pending = pe, proof_forest = pf,
+       pf_labels = pfl, input = ip\<rparr>
+                (rep_of l c\<^sub>2) c\<^sub>1 c\<^sub>2 c urest')" 
+    unfolding congruence_closure.select_convs by blast
+qed
 
 paragraph \<open>Invariants after the entire loop\<close>
 
 lemma lookup_invar_loop: 
   assumes "ufa_invar l"
-"lookup_invar \<lparr>cc_list = l, use_list = u, lookup = t, pending = pe, proof_forest = pf, pf_labels = pfl, input = ip\<rparr>"
+    "lookup_invar \<lparr>cc_list = l, use_list = u, lookup = t, pending = pe, proof_forest = pf, pf_labels = pfl, input = ip\<rparr>"
     (is "lookup_invar ?base") 
     "use_list_invar \<lparr>cc_list = l, use_list = u, lookup = t, pending = pe, proof_forest = pf, pf_labels = pfl, input = ip\<rparr>"
     "length t = length l" "length u = length l"
-"(\<forall> j < length u_a . use_list_valid_element (u_a ! j) l rep_b)"
-"rep_b < length l"
+    "(\<forall> j < length u_a . use_list_valid_element (u_a ! j) l rep_b)"
+    "rep_b < length l"
   shows "lookup_invar (propagate_loop rep_b u_a 
 \<lparr>cc_list = l, use_list = u, lookup = t, pending = pe, proof_forest = pf, pf_labels = pfl, input = ip\<rparr>
 )" 
   using assms proof(induction rep_b u_a 
-"\<lparr>cc_list = l, use_list = u, lookup = t, pending = pe, proof_forest = pf, pf_labels = pfl, input = ip\<rparr>"
-arbitrary: l u t pe pf pfl ip rule: propagate_loop.induct)
+    "\<lparr>cc_list = l, use_list = u, lookup = t, pending = pe, proof_forest = pf, pf_labels = pfl, input = ip\<rparr>"
+    arbitrary: l u t pe pf pfl ip rule: propagate_loop.induct)
   case (1 rep_b' u1' urest' l' u' t' pe' pf' pfl' ip')
   from "1.prems" have *: "\<forall>j<length urest'. use_list_valid_element (urest' ! j) l rep_b'" 
     by auto
   then show ?case proof(cases "lookup_Some t' l' u1'")
     case True
-with 1 have lookup_invar: "lookup_invar \<lparr>cc_list = l', use_list = u', lookup = t', pending = link_to_lookup t' l' u1' # pe',
+    with 1 have lookup_invar: "lookup_invar \<lparr>cc_list = l', use_list = u', lookup = t', pending = link_to_lookup t' l' u1' # pe',
                  proof_forest = pf', pf_labels = pfl', input = ip'\<rparr>" unfolding lookup_invar_def
       by auto
     from 1 have use_list_invar: "use_list_invar \<lparr>cc_list = l', use_list = u', lookup = t', pending = link_to_lookup t' l' u1' # pe',
                  proof_forest = pf', pf_labels = pfl', input = ip'\<rparr>" unfolding use_list_invar_def
-  by auto
+      by auto
     with 1 show ?thesis 
       using True * lookup_invar use_list_invar by auto
   next
     case False
     with "1.prems" obtain a\<^sub>1 a\<^sub>2 aa where u1': "u1' = (F a\<^sub>1 a\<^sub>2 \<approx> aa)"
-  "a\<^sub>1 < length l" "a\<^sub>2 < length l" "aa < length l" "rep_of l a\<^sub>1 = rep_b' \<or> rep_of l a\<^sub>2 = rep_b'"
+      "a\<^sub>1 < length l" "a\<^sub>2 < length l" "aa < length l" "rep_of l a\<^sub>1 = rep_b' \<or> rep_of l a\<^sub>2 = rep_b'"
       by (metis in_set_conv_nth list.set_intros(1))
     from 1 have lookup_invar: "lookup_invar \<lparr>cc_list = l', use_list = u'[rep_b' := u1' # u' ! rep_b'], lookup = update_lookup t' l' u1',
              pending = pe', proof_forest = pf', pf_labels = pfl', input = ip'\<rparr>" 
-  using lookup_invar_loop2 by auto
-  from 1 use_list_invar_loop2 u1' have use_list_invar: "use_list_invar \<lparr>cc_list = l', use_list = u'[rep_b' := u1' # u' ! rep_b'], lookup = update_lookup t' l' u1',
+      using lookup_invar_loop2 by auto
+    from 1 use_list_invar_loop2 u1' have use_list_invar: "use_list_invar \<lparr>cc_list = l', use_list = u'[rep_b' := u1' # u' ! rep_b'], lookup = update_lookup t' l' u1',
              pending = pe', proof_forest = pf', pf_labels = pfl', input = ip'\<rparr>" 
-    using congruence_closure.ext_inject by auto
-  with 1 show ?thesis 
+      using congruence_closure.ext_inject by auto
+    with 1 show ?thesis 
       using False * lookup_invar use_list_invar
       by (simp add: u1'(1))
   qed
@@ -385,49 +1031,49 @@ qed simp
 
 lemma pending_invar_loop: 
   assumes "ufa_invar l"
-"pending_invar \<lparr>cc_list = l, use_list = u, lookup = t, pending = pe, proof_forest = pf, pf_labels = pfl, input = ip\<rparr>" 
-"lookup_invar \<lparr>cc_list = l, use_list = u, lookup = t, pending = pe, proof_forest = pf, pf_labels = pfl, input = ip\<rparr>"
+    "pending_invar \<lparr>cc_list = l, use_list = u, lookup = t, pending = pe, proof_forest = pf, pf_labels = pfl, input = ip\<rparr>" 
+    "lookup_invar \<lparr>cc_list = l, use_list = u, lookup = t, pending = pe, proof_forest = pf, pf_labels = pfl, input = ip\<rparr>"
     "use_list_invar \<lparr>cc_list = l, use_list = u, lookup = t, pending = pe, proof_forest = pf, pf_labels = pfl, input = ip\<rparr>"
     "length t = length l" "length u = length l"
-"(\<forall> j < length u_a . use_list_valid_element (u_a ! j) l rep_b)"
-"rep_b < length l"
+    "(\<forall> j < length u_a . use_list_valid_element (u_a ! j) l rep_b)"
+    "rep_b < length l"
   shows "pending_invar (propagate_loop rep_b u_a 
 \<lparr>cc_list = l, use_list = u, lookup = t, pending = pe, proof_forest = pf, pf_labels = pfl, input = ip\<rparr>
 )" 
-using assms proof(induction rep_b u_a 
-"\<lparr>cc_list = l, use_list = u, lookup = t, pending = pe, proof_forest = pf, pf_labels = pfl, input = ip\<rparr>"
-arbitrary: l u t pe pf pfl ip  rule: propagate_loop.induct)
+  using assms proof(induction rep_b u_a 
+    "\<lparr>cc_list = l, use_list = u, lookup = t, pending = pe, proof_forest = pf, pf_labels = pfl, input = ip\<rparr>"
+    arbitrary: l u t pe pf pfl ip  rule: propagate_loop.induct)
   case (1 rep_b' u1' urest' l' u' t' pe' pf' pfl' ip')
   from "1.prems" obtain a\<^sub>1 a\<^sub>2 aa where u1': "u1' = (F a\<^sub>1 a\<^sub>2 \<approx> aa)"
-  "a\<^sub>1 < length l" "a\<^sub>2 < length l" "aa < length l" "rep_of l a\<^sub>1 = rep_b' \<or> rep_of l a\<^sub>2 = rep_b'"
+    "a\<^sub>1 < length l" "a\<^sub>2 < length l" "aa < length l" "rep_of l a\<^sub>1 = rep_b' \<or> rep_of l a\<^sub>2 = rep_b'"
     by (metis in_set_conv_nth list.set_intros(1))
-from 1 have *: "\<forall>j<length urest'. use_list_valid_element (urest' ! j) l' rep_b'" 
-      by auto
+  from 1 have *: "\<forall>j<length urest'. use_list_valid_element (urest' ! j) l' rep_b'" 
+    by auto
   show ?case proof(cases "lookup_Some t' l' u1'")
     case True
     with 1 u1' pending_invar_loop1 have pending_invar: "pending_invar \<lparr>cc_list = l', use_list = u', lookup = t', pending = link_to_lookup t' l' u1' # pe', proof_forest = pf',
              pf_labels = pfl', input = ip'\<rparr>" 
       by (metis congruence_closure.ext_inject)
-from 1 have lookup_invar: "lookup_invar \<lparr>cc_list = l', use_list = u', lookup = t', pending = link_to_lookup t' l' u1' # pe', proof_forest = pf',
+    from 1 have lookup_invar: "lookup_invar \<lparr>cc_list = l', use_list = u', lookup = t', pending = link_to_lookup t' l' u1' # pe', proof_forest = pf',
              pf_labels = pfl', input = ip'\<rparr>" unfolding lookup_invar_def 
-  by auto
-from 1 have use_list_invar: "use_list_invar \<lparr>cc_list = l', use_list = u', lookup = t', pending = link_to_lookup t' l' u1' # pe', proof_forest = pf',
+      by auto
+    from 1 have use_list_invar: "use_list_invar \<lparr>cc_list = l', use_list = u', lookup = t', pending = link_to_lookup t' l' u1' # pe', proof_forest = pf',
              pf_labels = pfl', input = ip'\<rparr>" unfolding use_list_invar_def 
-  by auto
-  with True pending_invar lookup_invar use_list_invar * show ?thesis using 1 
-    by simp
+      by auto
+    with True pending_invar lookup_invar use_list_invar * show ?thesis using 1 
+      by simp
   next
     case False
     from 1 have pending_invar: "pending_invar \<lparr>cc_list = l', use_list = u'[rep_b' := u1' # u' ! rep_b'], lookup = update_lookup t' l' u1', pending = pe',
              proof_forest = pf', pf_labels = pfl', input = ip'\<rparr>" 
       unfolding pending_invar_def 
       by fastforce
-from 1 lookup_invar_loop2 u1' have lookup_invar: "lookup_invar \<lparr>cc_list = l', use_list = u'[rep_b' := u1' # u' ! rep_b'], lookup = update_lookup t' l' u1', pending = pe',
+    from 1 lookup_invar_loop2 u1' have lookup_invar: "lookup_invar \<lparr>cc_list = l', use_list = u'[rep_b' := u1' # u' ! rep_b'], lookup = update_lookup t' l' u1', pending = pe',
              proof_forest = pf', pf_labels = pfl', input = ip'\<rparr>" 
-  by (metis congruence_closure.ext_inject)
-from 1 use_list_invar_loop2 u1' have use_list_invar: "use_list_invar \<lparr>cc_list = l', use_list = u'[rep_b' := u1' # u' ! rep_b'], lookup = update_lookup t' l' u1', pending = pe',
+      by (metis congruence_closure.ext_inject)
+    from 1 use_list_invar_loop2 u1' have use_list_invar: "use_list_invar \<lparr>cc_list = l', use_list = u'[rep_b' := u1' # u' ! rep_b'], lookup = update_lookup t' l' u1', pending = pe',
              proof_forest = pf', pf_labels = pfl', input = ip'\<rparr>" 
-  by (metis congruence_closure.ext_inject)
+      by (metis congruence_closure.ext_inject)
     with False pending_invar * show ?thesis using 1 
       using congruence_closure.ext_inject length_list_update lookup_invar propagate_loop.simps(1) u1'(1) update_lookup.simps(1) use_list_invar 
       by auto
@@ -436,23 +1082,23 @@ qed simp
 
 lemma use_list_invar_loop: 
   assumes "ufa_invar l" 
-"use_list_invar \<lparr>cc_list = l, use_list = u, lookup = t, pending = pe, proof_forest = pf, pf_labels = pfl, input = ip\<rparr>"
+    "use_list_invar \<lparr>cc_list = l, use_list = u, lookup = t, pending = pe, proof_forest = pf, pf_labels = pfl, input = ip\<rparr>"
     (is "use_list_invar ?base") 
-   "length u = length l"
-"(\<forall> j < length u_a . use_list_valid_element (u_a ! j) l rep_b)"
-"rep_b < length l"
+    "length u = length l"
+    "(\<forall> j < length u_a . use_list_valid_element (u_a ! j) l rep_b)"
+    "rep_b < length l"
   shows "use_list_invar (propagate_loop rep_b u_a 
 \<lparr>cc_list = l, use_list = u, lookup = t, pending = pe, proof_forest = pf, pf_labels = pfl, input = ip\<rparr>
 )" 
-using assms proof(induction rep_b u_a 
-"\<lparr>cc_list = l, use_list = u, lookup = t, pending = pe, proof_forest = pf, pf_labels = pfl, input = ip\<rparr>"
-arbitrary: l u t pe pf pfl ip  rule: propagate_loop.induct)
+  using assms proof(induction rep_b u_a 
+    "\<lparr>cc_list = l, use_list = u, lookup = t, pending = pe, proof_forest = pf, pf_labels = pfl, input = ip\<rparr>"
+    arbitrary: l u t pe pf pfl ip  rule: propagate_loop.induct)
   case (1 rep_b' u1' urest' l' u' t' pe' pf' pfl' ip')
   from "1.prems" obtain a\<^sub>1 a\<^sub>2 aa where u1': "u1' = (F a\<^sub>1 a\<^sub>2 \<approx> aa)"
-  "a\<^sub>1 < length l" "a\<^sub>2 < length l" "aa < length l" "rep_of l a\<^sub>1 = rep_b' \<or> rep_of l a\<^sub>2 = rep_b'"
+    "a\<^sub>1 < length l" "a\<^sub>2 < length l" "aa < length l" "rep_of l a\<^sub>1 = rep_b' \<or> rep_of l a\<^sub>2 = rep_b'"
     by (metis in_set_conv_nth list.set_intros(1))
-from 1 have *: "\<forall>j<length urest'. use_list_valid_element (urest' ! j) l' rep_b'" 
-      by auto
+  from 1 have *: "\<forall>j<length urest'. use_list_valid_element (urest' ! j) l' rep_b'" 
+    by auto
   show ?case proof(cases "lookup_Some t' l' u1'")
     case True
     from 1 have "use_list_invar \<lparr>cc_list = l', use_list = u', lookup = t', pending = link_to_lookup t' l' u1' # pe', proof_forest = pf',
@@ -462,39 +1108,238 @@ from 1 have *: "\<forall>j<length urest'. use_list_valid_element (urest' ! j) l'
       using "*" True by auto
   next
     case False
-from 1 u1' use_list_invar_loop2 have "use_list_invar \<lparr>cc_list = l', use_list = u'[rep_b' := u1' # u' ! rep_b'], lookup = update_lookup t' l' u1', pending = pe',
+    from 1 u1' use_list_invar_loop2 have "use_list_invar \<lparr>cc_list = l', 
+use_list = u'[rep_b' := u1' # u' ! rep_b'], lookup = update_lookup t' l' u1', pending = pe',
              proof_forest = pf', pf_labels = pfl', input = ip'\<rparr>" 
-  by (metis congruence_closure.ext_inject)
-  with 1 show ?thesis 
-    using "*" False by force
+      by (metis congruence_closure.ext_inject)
+    with 1 show ?thesis 
+      using "*" False by force
   qed
 qed simp
 
+lemma lookup_invar2_loop:
+  assumes 
+    "ufa_invar l" "a < length l" "b < length l"
+    "rep_of l a \<noteq> rep_of l b"
+    "lookup_invar2' \<lparr>cc_list = ufa_union l a b, 
+    use_list = u, 
+    lookup = t, 
+    pending = pe,
+    proof_forest = pf, 
+    pf_labels = pfl, 
+    input = ip\<rparr> u_a"
+
+    "\<forall> eq' \<in> set u_a . 
+(\<exists> c\<^sub>1 c\<^sub>2 c . eq' = (F c\<^sub>1 c\<^sub>2 \<approx> c) \<and> c\<^sub>1 < length l \<and> c\<^sub>2 < length l \<and> c < length l
+\<and> (rep_of l c\<^sub>1 \<noteq> rep_of l a \<longrightarrow> 
+contains_similar_equation \<lparr>cc_list = ufa_union l a b, 
+    use_list = u, 
+    lookup = t, 
+    pending = pe,
+    proof_forest = pf, 
+    pf_labels = pfl, 
+    input = ip\<rparr> (rep_of l c\<^sub>1) c\<^sub>1 c\<^sub>2 c u_a)
+
+\<and> 
+(rep_of l c\<^sub>2 \<noteq> rep_of l a \<longrightarrow> 
+contains_similar_equation \<lparr>cc_list = ufa_union l a b, 
+    use_list = u, 
+    lookup = t, 
+    pending = pe,
+    proof_forest = pf, 
+    pf_labels = pfl, 
+    input = ip\<rparr> (rep_of l c\<^sub>2) c\<^sub>1 c\<^sub>2 c u_a)
+)"
+    "(\<forall> j < length u_a . use_list_valid_element (u_a ! j) (ufa_union l a b) rep_b)"
+
+    "rep_b < length l"
+    "use_list_invar \<lparr>cc_list = ufa_union l a b, 
+    use_list = u, 
+    lookup = t, 
+    pending = pe,
+    proof_forest = pf, 
+    pf_labels = pfl, 
+    input = ip\<rparr>"
+    "lookup_invar \<lparr>cc_list = ufa_union l a b, 
+    use_list = u, 
+    lookup = t, 
+    pending = pe,
+    proof_forest = pf, 
+    pf_labels = pfl, 
+    input = ip\<rparr>"
+"length u = length l"
+"length l = length t"
+"rep_b = rep_of l b"
+"(\<forall> j < length u_a . use_list_valid_element (u_a ! j) l (rep_of l a))"
+  shows "lookup_invar2 (propagate_loop rep_b u_a 
+\<lparr>cc_list = ufa_union l a b, 
+    use_list = u, 
+    lookup = t, 
+    pending = pe,
+    proof_forest = pf, 
+    pf_labels = pfl, 
+    input = ip\<rparr>)"
+  using assms proof(induction rep_b u_a 
+    "\<lparr>cc_list = ufa_union l a b, use_list = u, lookup = t, pending = pe, 
+proof_forest = pf, pf_labels = pfl, input = ip\<rparr>"
+    arbitrary: u t pe rule: propagate_loop.induct)
+  case (1 rep_b' u1' urest' l' u' t' pe' pf' pfl' ip')
+  from 1(9) obtain c\<^sub>1 c\<^sub>2 c where u1': "u1' = (F c\<^sub>1 c\<^sub>2 \<approx> c)"
+    "c\<^sub>1 < length (ufa_union l a b)" "c\<^sub>2 < length (ufa_union l a b)" "c < length (ufa_union l a b)" 
+"rep_of (ufa_union l a b) c\<^sub>1 = rep_b' \<or> rep_of (ufa_union l a b) c\<^sub>2 = rep_b'"
+    by auto
+  then have c_length: "c\<^sub>1 < length l" "c\<^sub>2 < length l" "c < length l" 
+    using length_list_update 1(2) by simp_all
+ from 1(2) have eq: "l' = ufa_union l a b" "t = t'" "pe = pe'" by simp_all
+   show ?case proof(cases "lookup_entry t' l' c\<^sub>1 c\<^sub>2")
+    case None
+    let ?loop2 = "\<lparr>cc_list = ufa_union l a b, use_list = u[rep_b' := u1' # u ! rep_b'], 
+lookup = update_lookup t l' u1', 
+pending = pe, proof_forest = pf,
+       pf_labels = pfl, input = ip\<rparr>"
+
+    from None u1' eq have lookup_None: "\<not> lookup_Some t (ufa_union l a b) u1'" 
+      by fastforce
+    from 1(8) u1' have *: "(rep_of l c\<^sub>1 \<noteq> rep_of l a \<longrightarrow>
+     contains_similar_equation
+      \<lparr>cc_list = ufa_union l a b, use_list = u, lookup = t, pending = pe, proof_forest = pf,
+         pf_labels = pfl, input = ip\<rparr>
+      (rep_of l c\<^sub>1) c\<^sub>1 c\<^sub>2 c (u1' # urest')) \<and>
+    (rep_of l c\<^sub>2 \<noteq> rep_of l a \<longrightarrow>
+     contains_similar_equation
+      \<lparr>cc_list = ufa_union l a b, use_list = u, lookup = t, pending = pe, proof_forest = pf,
+         pf_labels = pfl, input = ip\<rparr>
+      (rep_of l c\<^sub>2) c\<^sub>1 c\<^sub>2 c (u1' # urest'))" 
+      by simp
+ from 1(16) obtain k\<^sub>1 k\<^sub>2 k where u1'': "u1' = (F k\<^sub>1 k\<^sub>2 \<approx> k)"
+    "k\<^sub>1 < length l" "k\<^sub>2 < length l" "k < length l" 
+"rep_of l k\<^sub>1 = rep_of l a \<or> rep_of l k\<^sub>2 = rep_of l a"
+    by auto
+    have "rep_b' < length u" " rep_b' = rep_of l b "
+      "rep_of l a = rep_of l c\<^sub>1 \<or> rep_of l a = rep_of l c\<^sub>2"
+      apply (simp add: "1.prems"(11) "1.prems"(8))
+       apply (simp add: "1.prems"(13))
+      using u1'' 
+      using u1'(1) by force
+    with lookup_invar2_loop2[OF assms(1,2,3) 1(11,12,7) assms(4) lookup_None u1'(1) c_length 1(14)
+_ *] 1(10,13) eq have 
+      2: "lookup_invar2' ?loop2 urest'"  
+      by blast
+    have *: "ufa_invar (ufa_union l a b)" "c\<^sub>1 < length (ufa_union l a b)" "c\<^sub>1 < length (ufa_union l a b)"
+      by (simp_all add: c_length assms(1) assms(2) assms(3) ufa_union_invar)
+    from lookup_invar2_prems_loop2[OF 1(8,12) _ _ lookup_None u1'(1,2,3,4)] eq  have 6: "\<forall>eq'\<in>set urest'.
+       \<exists>c\<^sub>1 c\<^sub>2 c.
+          eq' = (F c\<^sub>1 c\<^sub>2 \<approx> c) \<and>
+          c\<^sub>1 < length l \<and>
+          c\<^sub>2 < length l \<and>
+          c < length l \<and>
+          (rep_of l c\<^sub>1 \<noteq> rep_of l a \<longrightarrow>
+           contains_similar_equation
+            ?loop2
+            (rep_of l c\<^sub>1) c\<^sub>1 c\<^sub>2 c urest') \<and>
+          (rep_of l c\<^sub>2 \<noteq> rep_of l a \<longrightarrow>
+           contains_similar_equation
+            ?loop2
+            (rep_of l c\<^sub>2) c\<^sub>1 c\<^sub>2 c urest')"
+      using 1(14,10) "1.prems"(11) *(1) ufa_union_invar length_list_update 
+      by simp
+    from 1(9) have 3:"\<forall>j<length urest'. use_list_valid_element (urest' ! j) (ufa_union l a b) rep_b'"
+      by auto
+    have "rep_b' < length u" 
+      by (simp add: "1.prems"(11) "1.prems"(8))
+    then have 4: "use_list_invar ?loop2" "lookup_invar ?loop2" 
+      using 1(11) use_list_invar_loop2 u1' 
+      using \<open>l' = ufa_union l a b\<close> apply blast
+      using 1(12) lookup_invar_loop2 u1' 
+      using \<open>l' = ufa_union l a b\<close> by blast
+    from lookup_None 1(2) have 5: "(if lookup_Some t' l' u1'
+     then \<lparr>cc_list = l', use_list = u', lookup = t', pending = link_to_lookup t' l' u1' # pe',
+             proof_forest = pf', pf_labels = pfl', input = ip'\<rparr>
+     else \<lparr>cc_list = l', use_list = u'[rep_b' := u1' # u' ! rep_b'],
+             lookup = update_lookup t' l' u1', pending = pe', proof_forest = pf',
+             pf_labels = pfl', input = ip'\<rparr>) =
+    ?loop2" 
+      by auto
+    have " \<forall>j<length urest'. use_list_valid_element (urest' ! j) l (rep_of l a) " using 1(16) 
+      by auto
+    with 1(1)[OF 5(1) assms(1,2,3,4) 2 6 3 1(10) 4] "1.prems"(11,12) eq(1) lookup_None u1'(1) length_list_update
+    show ?thesis 
+      by (simp add: "1.prems"(13))
+  next
+    case (Some k)
+    let ?loop1 = "\<lparr>cc_list = ufa_union l a b, use_list = u, lookup = t, 
+pending = link_to_lookup t' l' u1' # pe', proof_forest = pf,
+       pf_labels = pfl, input = ip\<rparr>"
+    from Some u1' eq have lookup_Some: "lookup_Some t (ufa_union l a b) u1'" 
+      by fastforce
+    with lookup_invar2_loop1[OF assms(1,2,3) 1(11,12,7)] 1 u1' have 
+      2: "lookup_invar2' ?loop1 urest'" using c_length 
+      by blast
+    have *: "ufa_invar (ufa_union l a b)" "c\<^sub>1 < length (ufa_union l a b)" "c\<^sub>2 < length (ufa_union l a b)"
+      by (simp_all add: c_length assms(1) assms(2) assms(3) ufa_union_invar)
+   
+    with lookup_invar2_prems_loop1[OF 1(8,12) *(1) lookup_Some u1'(1) *(2,3)] have 6: "\<forall>eq'\<in>set urest'.
+       \<exists>c\<^sub>1 c\<^sub>2 c.
+          eq' = (F c\<^sub>1 c\<^sub>2 \<approx> c) \<and>
+          c\<^sub>1 < length l \<and>
+          c\<^sub>2 < length l \<and>
+          c < length l \<and>
+          (rep_of l c\<^sub>1 \<noteq> rep_of l a \<longrightarrow>
+           contains_similar_equation
+            ?loop1
+            (rep_of l c\<^sub>1) c\<^sub>1 c\<^sub>2 c urest') \<and>
+          (rep_of l c\<^sub>2 \<noteq> rep_of l a \<longrightarrow>
+           contains_similar_equation
+            ?loop1
+            (rep_of l c\<^sub>2) c\<^sub>1 c\<^sub>2 c urest')"
+      using eq by fastforce
+    from 1(9) have 3:"\<forall>j<length urest'. use_list_valid_element (urest' ! j) (ufa_union l a b) rep_b'"
+      by auto
+    have 4: "use_list_invar ?loop1" "lookup_invar ?loop1" 
+      using 1(11) unfolding use_list_invar_def apply simp
+      using 1(12) unfolding lookup_invar_def by simp
+    from lookup_Some 1(2) have 5: "(if lookup_Some t' l' u1'
+     then \<lparr>cc_list = l', use_list = u', lookup = t', pending = link_to_lookup t' l' u1' # pe',
+             proof_forest = pf', pf_labels = pfl', input = ip'\<rparr>
+     else \<lparr>cc_list = l', use_list = u'[rep_b' := u1' # u' ! rep_b'],
+             lookup = update_lookup t' l' u1', pending = pe', proof_forest = pf',
+             pf_labels = pfl', input = ip'\<rparr>) =
+    ?loop1" 
+      by auto
+have " \<forall>j<length urest'. use_list_valid_element (urest' ! j) l (rep_of l a) " using 1(16) 
+      by auto
+    with 1(1)[OF 5(1) assms(1,2,3,4) 2 6 3] 1(2-) 2 3 4 lookup_Some show ?thesis 
+      by auto
+  qed
+qed simp
+
+
 lemma inv2_loop: 
   assumes "a < length (cc_list cc)" "b < length (cc_list cc)" 
-"lookup_invar cc"
-"use_list_invar cc"
-"cc_list_invar cc"
-"length (use_list cc) = length (cc_list cc)"
-"length (lookup cc) = length (cc_list cc)"
-"(\<forall> j < length u_a . use_list_valid_element (u_a ! j) (cc_list cc) rep_b)"
-"rep_b < length (cc_list cc)"
-shows 
-"Congruence_Closure (representativeE cc \<union> pending_set (pending cc) \<union> set u_a) 
+    "lookup_invar cc"
+    "use_list_invar cc"
+    "cc_list_invar cc"
+    "length (use_list cc) = length (cc_list cc)"
+    "length (lookup cc) = length (cc_list cc)"
+    "(\<forall> j < length u_a . use_list_valid_element (u_a ! j) (cc_list cc) rep_b)"
+    "rep_b < length (cc_list cc)"
+    "rep_b = rep_of l b"
+  shows 
+    "Congruence_Closure (representativeE cc \<union> pending_set (pending cc) \<union> set u_a) 
 = Congruence_Closure (representativeE ((propagate_loop rep_b u_a cc)) 
 \<union> pending_set (pending (propagate_loop rep_b u_a cc)))" 
   using assms proof(induction rep_b u_a cc rule: propagate_loop.induct)
   case (1 rep_b' u1' urest' l' u' t' pe' pf' pfl' ip')
-from "1.prems" obtain a\<^sub>1 a\<^sub>2 aa where u1': "u1' = (F a\<^sub>1 a\<^sub>2 \<approx> aa)"
-  "a\<^sub>1 < length l'" "a\<^sub>2 < length l'" "aa < length l'" "rep_of l' a\<^sub>1 = rep_b' \<or> rep_of l' a\<^sub>2 = rep_b'"
-  unfolding congruence_closure.select_convs
-  by (metis in_set_conv_nth list.set_intros(1))
-from 1 have *: "\<forall>j<length urest'. use_list_valid_element (urest' ! j) l' rep_b'" 
-  by auto
-let ?loop1 = "\<lparr>cc_list = l', use_list = u', lookup = t',
+  from "1.prems" obtain a\<^sub>1 a\<^sub>2 aa where u1': "u1' = (F a\<^sub>1 a\<^sub>2 \<approx> aa)"
+    "a\<^sub>1 < length l'" "a\<^sub>2 < length l'" "aa < length l'" "rep_of l' a\<^sub>1 = rep_b' \<or> rep_of l' a\<^sub>2 = rep_b'"
+    unfolding congruence_closure.select_convs
+    by (metis in_set_conv_nth list.set_intros(1))
+  from 1 have *: "\<forall>j<length urest'. use_list_valid_element (urest' ! j) l' rep_b'" 
+    by auto
+  let ?loop1 = "\<lparr>cc_list = l', use_list = u', lookup = t',
                  pending = link_to_lookup t' l' u1' # pe', proof_forest = pf',
                  pf_labels = pfl', input = ip'\<rparr>"
-let ?loop2 = "\<lparr>cc_list = l', use_list = u'[rep_b' := u1' # u' ! rep_b'],
+  let ?loop2 = "\<lparr>cc_list = l', use_list = u'[rep_b' := u1' # u' ! rep_b'],
                 lookup = update_lookup t' l' u1', pending = pe',
                 proof_forest = pf', pf_labels = pfl', input = ip'\<rparr>"
   let ?step = "if lookup_Some t' l' u1'
@@ -529,7 +1374,7 @@ let ?loop2 = "\<lparr>cc_list = l', use_list = u'[rep_b' := u1' # u' ! rep_b'],
     case False
     have invars: "lookup_invar ?loop2" "use_list_invar ?loop2" 
       using "1.prems"(3,4) lookup_invar_loop2 u1' 
-      apply blast using "1.prems" use_list_invar_loop2 u1' by force
+       apply blast using "1.prems" use_list_invar_loop2 u1' by force
     with 1 have **: "Congruence_Closure
      (representativeE ?loop2 \<union> pending_set (pending ?loop2) \<union>
       set urest') = Congruence_Closure (representativeE
@@ -559,19 +1404,19 @@ paragraph \<open>Invariants before entering the propagate_loop.\<close>
 
 lemma lookup_invar_mini_step:
   assumes "lookup_invar \<lparr>cc_list = l, use_list = u, lookup = t, pending = (eq # pe), proof_forest = pf, pf_labels = pfl, input = ip\<rparr>"
-(is "lookup_invar ?base") "ufa_invar l" "a < length l" "b < length l"
-shows "lookup_invar \<lparr>cc_list = ufa_union l a b,
+    (is "lookup_invar ?base") "ufa_invar l" "a < length l" "b < length l"
+  shows "lookup_invar \<lparr>cc_list = ufa_union l a b,
     use_list = u[rep_of l a := []], 
     lookup = t, 
     pending = pe,
     proof_forest = add_edge pf a b, 
     pf_labels = add_label pfl pf a eq, 
     input = ip\<rparr>" (is "lookup_invar ?step")  
-unfolding lookup_invar_def
+  unfolding lookup_invar_def
 proof(standard, standard, standard, standard, standard, standard)
   fix i j
   assume i_j: "i < nr_vars ?step" "j < nr_vars ?step"
-"cc_list ?step ! i = i \<and> cc_list ?step ! j = j"
+    "cc_list ?step ! i = i \<and> cc_list ?step ! j = j"
   then have "cc_list ?base ! i = i \<and> cc_list ?base ! j = j" 
     by (metis assms(2) assms(3) assms(4) congruence_closure.select_convs(1) ufa_union_root)
   with assms i_j show "lookup_valid_element (lookup ?step) (cc_list ?step) i j"
@@ -585,20 +1430,20 @@ qed
 
 lemma use_list_invar_mini_step:
   assumes "use_list_invar \<lparr>cc_list = l, use_list = u, lookup = t, pending = (eq # pe), proof_forest = pf, pf_labels = pfl, input = ip\<rparr>"
-(is "use_list_invar ?base") "ufa_invar l" "a < length l" "b < length l" "length l = length u"
-shows "use_list_invar \<lparr>cc_list = ufa_union l a b,
+    (is "use_list_invar ?base") "ufa_invar l" "a < length l" "b < length l" "length l = length u"
+  shows "use_list_invar \<lparr>cc_list = ufa_union l a b,
     use_list = u[rep_of l a := []], 
     lookup = t, 
     pending = pe,
     proof_forest = add_edge pf a b, 
     pf_labels = add_label pfl pf a eq, 
     input = ip\<rparr>" (is "use_list_invar ?step")  
-unfolding use_list_invar_def
+  unfolding use_list_invar_def
 proof(standard, standard, standard, standard, standard)
   fix i j
   assume i_j: "i < nr_vars ?step" "j < length (use_list ?step ! i)" "cc_list ?step ! i = i"
-then have "cc_list ?base ! i = i" 
-  by (metis assms(2) assms(3) assms(4) congruence_closure.select_convs(1) ufa_union_root)
+  then have "cc_list ?base ! i = i" 
+    by (metis assms(2) assms(3) assms(4) congruence_closure.select_convs(1) ufa_union_root)
   have "rep_of l a < length u" 
     by (metis assms(2) assms(3) assms(5) rep_of_bound)
   then show "use_list_valid_element (use_list ?step ! i ! j) (cc_list ?step) i"
@@ -610,20 +1455,20 @@ then have "cc_list ?base ! i = i"
       using i_j(2) by presburger
   next
     case False
-then have "(use_list ?step ! i) = (use_list ?base ! i)" 
-  by fastforce
-  with assms show ?thesis unfolding use_list_invar_def 
-    by (metis \<open>cc_list \<lparr>cc_list = l, use_list = u, lookup = t, pending = (eq # pe), proof_forest = pf, pf_labels = pfl, input = ip\<rparr> ! i = i\<close> congruence_closure.select_convs(1) i_j(1) i_j(2) i_j(3) length_list_update rep_of_iff rep_of_ufa_union_invar ufa_union_invar)
+    then have "(use_list ?step ! i) = (use_list ?base ! i)" 
+      by fastforce
+    with assms show ?thesis unfolding use_list_invar_def 
+      by (metis \<open>cc_list \<lparr>cc_list = l, use_list = u, lookup = t, pending = (eq # pe), proof_forest = pf, pf_labels = pfl, input = ip\<rparr> ! i = i\<close> congruence_closure.select_convs(1) i_j(1) i_j(2) i_j(3) length_list_update rep_of_iff rep_of_ufa_union_invar ufa_union_invar)
   qed
 qed
 
 
 lemma pending_invar_mini_step:
-assumes "ufa_invar l" "a < length l" "b < length l"
-"pending_invar \<lparr>cc_list = l, use_list = u, lookup = t, pending = (eq2 # pe), 
+  assumes "ufa_invar l" "a < length l" "b < length l"
+    "pending_invar \<lparr>cc_list = l, use_list = u, lookup = t, pending = (eq2 # pe), 
 proof_forest = pf, pf_labels = pfl, input = ip\<rparr>"
-(is "pending_invar ?base")
-shows"pending_invar \<lparr>cc_list = ufa_union l a b, 
+    (is "pending_invar ?base")
+  shows"pending_invar \<lparr>cc_list = ufa_union l a b, 
     use_list = u[rep_of l a := []], 
     lookup = t, 
     pending = pe,
@@ -646,7 +1491,7 @@ proof(standard, standard)
   next
     case (Two a\<^sub>1 a\<^sub>2 a' b\<^sub>1 b\<^sub>2 b')
     with * have "rep_of (ufa_union l a b) a\<^sub>1 = rep_of (ufa_union l a b) b\<^sub>1"
- "rep_of (ufa_union l a b) a\<^sub>2 = rep_of (ufa_union l a b) b\<^sub>2"
+      "rep_of (ufa_union l a b) a\<^sub>2 = rep_of (ufa_union l a b) b\<^sub>2"
       unfolding congruence_closure.select_convs
       by (metis assms(1) assms(2) assms(3) rep_of_ufa_union_invar)+
     with * Two show ?case 
@@ -785,8 +1630,8 @@ proof(induction rule: Congruence_Closure_eq)
     have "rep_of l a < length l" "l ! (rep_of l a) = rep_of l a" 
        apply (simp add: assms(1) assms(2) rep_of_less_length_l)
       by (simp add: assms(1) assms(2) rep_of_min)
-    with assms urest show ?thesis unfolding use_list_invar2_def congruence_closure.select_convs 
-      by blast
+    with assms urest show ?thesis unfolding  congruence_closure.select_convs 
+      sorry
   qed 
 next
   case (right eq)
@@ -811,8 +1656,8 @@ next
     then show ?thesis proof(cases "a' = rep_of l a \<or> b' = rep_of l a")
       case True
       with assms lookup have  "(F c\<^sub>1 c\<^sub>2 \<approx> c) \<in> set (u ! rep_of l a)"
-        unfolding lookup_invar2_def congruence_closure.select_convs 
-        by blast
+        unfolding lookup_invar2'_def congruence_closure.select_convs 
+        sorry
       then have cc1: "Congruence_Closure (representativeE ?step \<union> pending_set pe \<union> set (u ! rep_of l a))
 (F c\<^sub>1 c\<^sub>2 \<approx> c)"
         using Congruence_Closure_split_rule by blast
@@ -854,27 +1699,159 @@ next
       with ** transitive2 Congruence_Closure_union show ?thesis 
         using lookup(1) by blast
     qed
-next
-  case new_eq
-  with assms have "valid_vars_pending eq2 l" unfolding pending_invar_def 
-    by fastforce
-  with new_eq have eq: "eq = (a \<approx> b)"
-    by (simp add: assms(4) assms(5))
-  have "rep_of (ufa_union l a b) a = rep_of (ufa_union l a b) b" 
-    by (simp add: assms(1) assms(2) assms(3) ufa_union_aux)
-  then have "Congruence_Closure (representativeE ?step) (a \<approx> b)"
-    using CC_same_rep assms by auto
-  then show ?thesis using Congruence_Closure_union eq 
-    by blast
-qed (simp add: base)
+  next
+    case new_eq
+    with assms have "valid_vars_pending eq2 l" unfolding pending_invar_def 
+      by fastforce
+    with new_eq have eq: "eq = (a \<approx> b)"
+      by (simp add: assms(4) assms(5))
+    have "rep_of (ufa_union l a b) a = rep_of (ufa_union l a b) b" 
+      by (simp add: assms(1) assms(2) assms(3) ufa_union_aux)
+    then have "Congruence_Closure (representativeE ?step) (a \<approx> b)"
+      using CC_same_rep assms by auto
+    then show ?thesis using Congruence_Closure_union eq 
+      by blast
+  qed (simp add: base)
 qed
+
+lemma lookup_invar2_mini_step:
+  assumes "lookup_invar2 \<lparr>cc_list = l, use_list = u, lookup = t, pending = (eq # pe), 
+proof_forest = pf, pf_labels = pfl, input = ip\<rparr>"
+    (is "lookup_invar2 ?base")
+    "use_list_invar \<lparr>cc_list = l, use_list = u, lookup = t, pending = (eq # pe), 
+proof_forest = pf, pf_labels = pfl, input = ip\<rparr>"
+    "use_list_invar2 \<lparr>cc_list = l, use_list = u, lookup = t, pending = (eq # pe), 
+proof_forest = pf, pf_labels = pfl, input = ip\<rparr>"
+    "lookup_invar \<lparr>cc_list = l, use_list = u, lookup = t, pending = (eq # pe), 
+proof_forest = pf, pf_labels = pfl, input = ip\<rparr>"
+    "pending_invar \<lparr>cc_list = l, use_list = u, lookup = t, pending = (eq # pe), 
+proof_forest = pf, pf_labels = pfl, input = ip\<rparr>"
+    "ufa_invar l" "a < length l" "b < length l"
+    "a = left eq" "b = right eq"
+    "rep_of l a \<noteq> rep_of l b"
+  shows "lookup_invar2' \<lparr>cc_list = ufa_union l a b, 
+    use_list = u[rep_of l a := []], 
+    lookup = t, 
+    pending = pe,
+    proof_forest = add_edge pf a b, 
+    pf_labels = add_label pfl pf a eq, 
+    input = ip\<rparr> (u ! rep_of l a)"
+    (is "lookup_invar2' ?mini_step (u ! rep_of l a)")
+  unfolding lookup_invar2'_def congruence_closure.select_convs
+proof(standard, standard, standard, standard, standard, standard, standard, standard, standard, standard)
+  fix a' b' c c\<^sub>1 c\<^sub>2
+  assume prems: "a' < length (ufa_union l a b)"
+    "b' < length (ufa_union l a b)"
+    "ufa_union l a b ! a' = a'"
+    "ufa_union l a b ! b' = b'"
+    "t ! a' ! b' = Some (F c\<^sub>1 c\<^sub>2 \<approx> c)"
+  with assms have *: "l ! a' = a'" "l ! b' = b'" "a' < length l" "b' < length l"
+    "t ! a' ! b' = Some (F c\<^sub>1 c\<^sub>2 \<approx> c)"
+    using ufa_union_root apply blast+ 
+    using prems by auto
+  with assms obtain b\<^sub>1 b\<^sub>2 bc a\<^sub>1 a\<^sub>2 ac where 1: "
+         (F b\<^sub>1 b\<^sub>2 \<approx> bc) \<in> set (u ! b') \<and>
+         rep_of l b\<^sub>1 = rep_of l c\<^sub>1 \<and>
+         rep_of l b\<^sub>2 = rep_of l c\<^sub>2 \<and>
+         Congruence_Closure
+          (representativeE
+            \<lparr>cc_list = l, use_list = u, lookup = t, pending = eq # pe, proof_forest = pf,
+               pf_labels = pfl, input = ip\<rparr> \<union>
+           pending_set (eq # pe))
+          (bc \<approx> c)"
+    "
+         (F a\<^sub>1 a\<^sub>2 \<approx> ac) \<in> set (u ! a') \<and>
+         rep_of l a\<^sub>1 = rep_of l c\<^sub>1 \<and>
+         rep_of l a\<^sub>2 = rep_of l c\<^sub>2 \<and>
+         Congruence_Closure
+          (representativeE
+            \<lparr>cc_list = l, use_list = u, lookup = t, pending = eq # pe, proof_forest = pf,
+               pf_labels = pfl, input = ip\<rparr> \<union>
+           pending_set (eq # pe))
+          (ac \<approx> c)" unfolding lookup_invar2'_def congruence_closure.select_convs
+    by fastforce
+  have 4: "aa < length l \<Longrightarrow> bb < length l \<Longrightarrow> 
+rep_of l aa = rep_of l bb \<Longrightarrow> rep_of (ufa_union l a b) aa = rep_of (ufa_union l a b) bb" 
+    for aa bb using assms rep_of_ufa_union_invar by blast
+  from assms use_list_invar_less_n_in_set * 1
+  have 5: "b\<^sub>1 < length l" "b\<^sub>2 < length l" "bc < length l"
+    "a\<^sub>1 < length l" "a\<^sub>2 < length l" "ac < length l"
+    by metis+
+  from inv2_mini_step 
+    assms have 6: "Congruence_Closure
+          (representativeE
+            \<lparr>cc_list = l, use_list = u, lookup = t, pending = eq # pe, proof_forest = pf,
+               pf_labels = pfl, input = ip\<rparr> \<union>
+           pending_set (eq # pe)) 
+= Congruence_Closure
+         (representativeE
+              \<lparr>cc_list = ufa_union l a b, use_list = u[rep_of l a := []], lookup = t, pending = pe,
+                 proof_forest = add_edge pf a b, pf_labels = add_label pfl pf a eq, input = ip\<rparr> \<union>
+             pending_set pe \<union> set (u ! rep_of l a))" 
+    by force
+  from assms prems * have "a' \<noteq> rep_of l a" "b' \<noteq> rep_of l a"
+    by (metis nth_list_update_eq)+
+  then have 3: "u[rep_of l a := []] ! a' = u ! a'"
+    "u[rep_of l a := []] ! b' = u ! b'"
+    by fastforce+
+  from assms * lookup_invar_less_n
+  have "c\<^sub>1 < length l" "c\<^sub>2 < length l" "c < length l"
+    by simp_all
+  with 1 4 5 6 * have "
+           ((F b\<^sub>1 b\<^sub>2 \<approx> bc) \<in> set (u[rep_of l a := []] ! b') \<and>
+           rep_of (ufa_union l a b) b\<^sub>1 = rep_of (ufa_union l a b) c\<^sub>1 \<and>
+           rep_of (ufa_union l a b) b\<^sub>2 = rep_of (ufa_union l a b) c\<^sub>2 \<and>
+           Congruence_Closure
+            (representativeE
+              \<lparr>cc_list = ufa_union l a b, use_list = u[rep_of l a := []], lookup = t, pending = pe,
+                 proof_forest = add_edge pf a b, pf_labels = add_label pfl pf a eq, input = ip\<rparr> \<union>
+             pending_set pe \<union> set (u ! rep_of l a))
+            (bc \<approx> c))
+       ""
+           (F a\<^sub>1 a\<^sub>2 \<approx> ac) \<in> set (u[rep_of l a := []] ! a') \<and>
+           rep_of (ufa_union l a b) a\<^sub>1 = rep_of (ufa_union l a b) c\<^sub>1 \<and>
+           rep_of (ufa_union l a b) a\<^sub>2 = rep_of (ufa_union l a b) c\<^sub>2 \<and>
+           Congruence_Closure
+            (representativeE
+              \<lparr>cc_list = ufa_union l a b, use_list = u[rep_of l a := []], lookup = t, pending = pe,
+                 proof_forest = add_edge pf a b, pf_labels = add_label pfl pf a eq, input = ip\<rparr> \<union>
+             pending_set pe \<union> set (u ! rep_of l a))
+            (ac \<approx> c)" unfolding 6 3
+    by blast+
+  then show "(\<exists>b\<^sub>1 b\<^sub>2 ba.
+           (F b\<^sub>1 b\<^sub>2 \<approx> ba) \<in> set (u[rep_of l a := []] ! a') \<and>
+           rep_of (ufa_union l a b) b\<^sub>1 = rep_of (ufa_union l a b) c\<^sub>1 \<and>
+           rep_of (ufa_union l a b) b\<^sub>2 = rep_of (ufa_union l a b) c\<^sub>2 \<and>
+           Congruence_Closure
+            (representativeE
+              \<lparr>cc_list = ufa_union l a b, use_list = u[rep_of l a := []], lookup = t,
+                 pending = pe, proof_forest = add_edge pf a b,
+                 pf_labels = add_label pfl pf a eq, input = ip\<rparr> \<union>
+             pending_set pe \<union>
+             set (u ! rep_of l a))
+            (ba \<approx> c)) \<and>
+       (\<exists>b\<^sub>1 b\<^sub>2 ba.
+           (F b\<^sub>1 b\<^sub>2 \<approx> ba) \<in> set (u[rep_of l a := []] ! b') \<and>
+           rep_of (ufa_union l a b) b\<^sub>1 = rep_of (ufa_union l a b) c\<^sub>1 \<and>
+           rep_of (ufa_union l a b) b\<^sub>2 = rep_of (ufa_union l a b) c\<^sub>2 \<and>
+           Congruence_Closure
+            (representativeE
+              \<lparr>cc_list = ufa_union l a b, use_list = u[rep_of l a := []], lookup = t,
+                 pending = pe, proof_forest = add_edge pf a b,
+                 pf_labels = add_label pfl pf a eq, input = ip\<rparr> \<union>
+             pending_set pe \<union>
+             set (u ! rep_of l a))
+            (ba \<approx> c)) "
+    by auto
+qed
+
 
 paragraph \<open>Invariants after one step of propagate\<close>
 
 lemma proof_forest_invar_step: 
   assumes "ufa_invar l" "a < length l" "b < length l" "length l = length pf"
-"proof_forest_invar \<lparr>cc_list = l, use_list = u, lookup = t, pending = (eq # pe), proof_forest = pf, pf_labels = pfl, input = ip\<rparr>"
-   "rep_of pf a \<noteq> rep_of pf b"
+    "proof_forest_invar \<lparr>cc_list = l, use_list = u, lookup = t, pending = (eq # pe), proof_forest = pf, pf_labels = pfl, input = ip\<rparr>"
+    "rep_of pf a \<noteq> rep_of pf b"
   shows "proof_forest_invar (propagate_step l u t pe pf pfl ip a b eq)"
   using assms proof(induction rule: propagate_step_induct)
   case base
@@ -884,7 +1861,7 @@ qed (simp_all add: proof_forest_invar_def)
 
 lemma inv_same_rep_classes_step:
   assumes  "ufa_invar l" "a < length l" "b < length l"
-"inv_same_rep_classes \<lparr>cc_list = l, use_list = u, lookup = t, pending = (eq # pe), proof_forest = pf, pf_labels = pfl, input = ip\<rparr>"
+    "inv_same_rep_classes \<lparr>cc_list = l, use_list = u, lookup = t, pending = (eq # pe), proof_forest = pf, pf_labels = pfl, input = ip\<rparr>"
     (is "inv_same_rep_classes ?base")
     "rep_of pf a \<noteq> rep_of pf b" "ufa_invar pf" "length pf = length l"
   shows "inv_same_rep_classes (propagate_step l u t pe pf pfl ip a b eq)"
@@ -895,30 +1872,30 @@ lemma inv_same_rep_classes_step:
     fix i j
     let ?step = "\<lparr>cc_list = ufa_union l a b, use_list = u[rep_of l a := []], lookup = t, pending = pe,
                      proof_forest = add_edge pf a b, pf_labels = add_label pfl pf a eq, input = ip\<rparr>"
-  assume i_j: "i < length (proof_forest ?step)" "j < length (proof_forest ?step)"
-  with add_edge_preserves_length' assms have *:"length (proof_forest ?step) = length (proof_forest ?base)" 
-    by simp
-  with add_edge_preserves_length' assms have "length (cc_list ?step) = length (cc_list ?base)" 
-    by simp
-  with assms * have "(rep_of (cc_list ?base) i = rep_of (cc_list ?base) j) =
+    assume i_j: "i < length (proof_forest ?step)" "j < length (proof_forest ?step)"
+    with add_edge_preserves_length' assms have *:"length (proof_forest ?step) = length (proof_forest ?base)" 
+      by simp
+    with add_edge_preserves_length' assms have "length (cc_list ?step) = length (cc_list ?base)" 
+      by simp
+    with assms * have "(rep_of (cc_list ?base) i = rep_of (cc_list ?base) j) =
            (rep_of (proof_forest ?base) i = rep_of (proof_forest ?base) j)" unfolding inv_same_rep_classes_def using inv_same_rep_classes_not_divided 
-    using i_j by presburger
-  \<comment>\<open>The representative classes of add_edge and ufa_invar have the same behaviour\<close>
-  with rep_of_add_edge_aux ufa_union_aux 
-  show "(rep_of (cc_list ?step) i = rep_of (cc_list ?step) j) =
+      using i_j by presburger
+        \<comment>\<open>The representative classes of add_edge and ufa_invar have the same behaviour\<close>
+    with rep_of_add_edge_aux ufa_union_aux 
+    show "(rep_of (cc_list ?step) i = rep_of (cc_list ?step) j) =
            (rep_of (proof_forest ?step) i = rep_of (proof_forest ?step) j) " 
-    using assms * i_j inv_same_rep_classes_not_divided unfolding congruence_closure.select_convs 
-    by (smt (z3) congruence_closure.select_convs(1) congruence_closure.select_convs(5))
-qed
+      using assms * i_j inv_same_rep_classes_not_divided unfolding congruence_closure.select_convs 
+      by (smt (z3) congruence_closure.select_convs(1) congruence_closure.select_convs(5))
+  qed
 qed auto
 
 lemma use_list_invar_impl_valid_input_propagate_loop:
   assumes "ufa_invar l" "a < length l" "b < length l" 
-"use_list_invar \<lparr>cc_list = l, use_list = u, lookup = t, pending = (eq # pe), proof_forest = pf, pf_labels = pfl, input = ip\<rparr>"
+    "use_list_invar \<lparr>cc_list = l, use_list = u, lookup = t, pending = (eq # pe), proof_forest = pf, pf_labels = pfl, input = ip\<rparr>"
   shows "(\<forall> j < length (u ! rep_of l a) . use_list_valid_element ((u ! rep_of l a) ! j) (ufa_union l a b) (rep_of l b))"
-"(rep_of l b) < length l"
+    "(rep_of l b) < length l"
 proof-
-have "rep_of l a < length l" "l ! rep_of l a = rep_of l a"
+  have "rep_of l a < length l" "l ! rep_of l a = rep_of l a"
     by (simp_all add: assms(1) assms(2) rep_of_less_length_l rep_of_root)
   with assms have"(\<forall> j < length (u ! rep_of l a) . use_list_valid_element ((u ! rep_of l a) ! j) l (rep_of l a))"
     unfolding use_list_invar_def
@@ -926,13 +1903,142 @@ have "rep_of l a < length l" "l ! rep_of l a = rep_of l a"
   moreover have "rep_of (ufa_union l a b) a = rep_of l b"
     by (simp add: assms(1) assms(2) assms(3) ufa_union_aux)
   ultimately show "(\<forall> j < length (u ! rep_of l a) . use_list_valid_element ((u ! rep_of l a) ! j) (ufa_union l a b) (rep_of l b))"
-"(rep_of l b) < length l" unfolding use_list_invar_def
+    "(rep_of l b) < length l" unfolding use_list_invar_def
     using assms(1) assms(3) ufa_union_aux rep_of_less_length_l by auto
+qed
+
+lemma lookup2_invar_impl_valid_input_propagate_loop:
+  assumes "lookup_invar2 \<lparr>cc_list = l, use_list = u, lookup = t, pending = (eq # pe), 
+proof_forest = pf, pf_labels = pfl, input = ip\<rparr>"
+    (is "lookup_invar2 ?base")
+    "use_list_invar \<lparr>cc_list = l, use_list = u, lookup = t, pending = (eq # pe), 
+proof_forest = pf, pf_labels = pfl, input = ip\<rparr>"
+    "use_list_invar2 \<lparr>cc_list = l, use_list = u, lookup = t, pending = (eq # pe), 
+proof_forest = pf, pf_labels = pfl, input = ip\<rparr>"
+    "lookup_invar \<lparr>cc_list = l, use_list = u, lookup = t, pending = (eq # pe), 
+proof_forest = pf, pf_labels = pfl, input = ip\<rparr>"
+    "pending_invar \<lparr>cc_list = l, use_list = u, lookup = t, pending = (eq # pe), 
+proof_forest = pf, pf_labels = pfl, input = ip\<rparr>"
+    "ufa_invar l" "a < length l" "b < length l"
+    "a = left eq" "b = right eq"
+    "rep_of l a \<noteq> rep_of l b"
+  shows "\<forall> eq' \<in> set (u ! rep_of l a) . 
+(\<exists> c\<^sub>1 c\<^sub>2 c . eq' = (F c\<^sub>1 c\<^sub>2 \<approx> c) \<and> c\<^sub>1 < length l \<and> c\<^sub>2 < length l \<and> c < length l
+\<and> (rep_of l c\<^sub>1 \<noteq> rep_of l a \<longrightarrow> 
+contains_similar_equation \<lparr>cc_list = ufa_union l a b, 
+    use_list = u[rep_of l a := []], 
+    lookup = t, 
+    pending = pe,
+    proof_forest = add_edge pf a b, 
+    pf_labels = add_label pfl pf a eq, 
+    input = ip\<rparr> (rep_of l c\<^sub>1) c\<^sub>1 c\<^sub>2 c (u ! rep_of l a))
+
+\<and> 
+(rep_of l c\<^sub>2 \<noteq> rep_of l a \<longrightarrow> 
+contains_similar_equation \<lparr>cc_list = ufa_union l a b, 
+    use_list = u[rep_of l a := []], 
+    lookup = t, 
+    pending = pe,
+    proof_forest = add_edge pf a b, 
+    pf_labels = add_label pfl pf a eq, 
+    input = ip\<rparr> (rep_of l c\<^sub>2) c\<^sub>1 c\<^sub>2 c (u ! rep_of l a))
+)"
+proof(standard)
+  fix eq'
+  assume eq': "eq' \<in> set (u ! rep_of l a)"
+  with assms use_list_invar_less_n_in_set'
+  obtain c\<^sub>1 c\<^sub>2 c where c: "eq' = (F c\<^sub>1 c\<^sub>2 \<approx> c)"
+    "c\<^sub>1 < length l" "c\<^sub>2 < length l" "c < length l" 
+    by (metis rep_of_bound rep_of_root use_list_invar_less_n_in_set(1))
+  with assms obtain b\<^sub>1 b\<^sub>2 bb where 
+    b: "lookup_entry t l c\<^sub>1 c\<^sub>2 = Some (F b\<^sub>1 b\<^sub>2 \<approx> bb)" 
+    "Congruence_Closure (representativeE ?base \<union> pending_set (pending ?base)
+                  \<union> set []) (bb \<approx> c)"
+    unfolding use_list_invar2'_def 
+    by (metis eq' congruence_closure.select_convs(1-3) rep_of_bound rep_of_min)
+  with assms c rep_of_bound rep_of_min
+  have *: "rep_of l c\<^sub>1 < length l" "l ! rep_of l c\<^sub>1 = rep_of l c\<^sub>1" 
+    "rep_of l c\<^sub>2 < length l" "l ! rep_of l c\<^sub>2 = rep_of l c\<^sub>2" 
+    "lookup_entry t l c\<^sub>1 c\<^sub>2 \<noteq> None"
+    by auto
+  with assms have c_eq_b: "rep_of l c\<^sub>1 = rep_of l b\<^sub>1" "rep_of l c\<^sub>2 = rep_of l b\<^sub>2"
+    unfolding lookup_invar_def congruence_closure.select_convs 
+    by (metis b(1) equation.inject(2) option.inject)+
+  with assms * c b obtain d\<^sub>1 d\<^sub>2 d where d: "(F d\<^sub>1 d\<^sub>2 \<approx> d) \<in> set (u ! rep_of l b\<^sub>2)"
+    "rep_of l d\<^sub>1 = rep_of l b\<^sub>1" 
+    "rep_of l d\<^sub>2 = rep_of l b\<^sub>2"
+    "Congruence_Closure (representativeE ?base \<union> pending_set (eq # pe)
+            \<union> set []) (d \<approx> bb)"
+    unfolding lookup_invar2'_def congruence_closure.select_convs by metis
+  with b(2) transitive1 have CC_d_c: "Congruence_Closure (representativeE ?base \<union> pending_set (eq # pe)
+            \<union> set []) (d \<approx> c)" 
+    unfolding congruence_closure.select_convs by blast
+  from c_eq_b * assms c d have c2_step: "rep_of l a \<noteq> rep_of l c\<^sub>2 \<Longrightarrow> 
+(F d\<^sub>1 d\<^sub>2 \<approx> d) \<in> set ((u[rep_of l a := []]) ! rep_of (ufa_union l a b) c\<^sub>2) \<and> 
+rep_of (ufa_union l a b) d\<^sub>1 = rep_of (ufa_union l a b) c\<^sub>1 \<and> 
+rep_of (ufa_union l a b) d\<^sub>2 = rep_of (ufa_union l a b) c\<^sub>2"
+    by (metis ufa_union_aux nth_list_update_neq rep_of_ufa_union_invar use_list_invar_less_n_in_set(1,2))
+  have CC_step: "Congruence_Closure (representativeE ?base \<union> pending_set (eq # pe)
+            \<union> set []) = Congruence_Closure (representativeE \<lparr>cc_list = ufa_union l a b, 
+    use_list = u[rep_of l a := []], 
+    lookup = t, 
+    pending = pe,
+    proof_forest = add_edge pf a b, 
+    pf_labels = add_label pfl pf a eq, 
+    input = ip\<rparr> \<union> pending_set pe
+            \<union> set (u ! rep_of l a))" 
+    using assms inv2_mini_step by simp
+  with assms * c b c_eq_b obtain e\<^sub>1 e\<^sub>2 e where e: "(F e\<^sub>1 e\<^sub>2 \<approx> e) \<in> set (u ! rep_of l b\<^sub>1)"
+    "rep_of l e\<^sub>1 = rep_of l b\<^sub>1" 
+    "rep_of l e\<^sub>2 = rep_of l b\<^sub>2"
+    "Congruence_Closure (representativeE ?base \<union> pending_set (eq # pe)
+            \<union> set []) (e \<approx> bb)"
+    unfolding lookup_invar2'_def congruence_closure.select_convs by metis
+  with b(2) transitive1 have CC_e_c: "Congruence_Closure (representativeE ?base \<union> pending_set (eq # pe)
+            \<union> set []) (e \<approx> c)" 
+    unfolding congruence_closure.select_convs by blast
+  from e c_eq_b * assms c have c1_step: "rep_of l a \<noteq> rep_of l c\<^sub>1 \<Longrightarrow> 
+(F e\<^sub>1 e\<^sub>2 \<approx> e) \<in> set ((u[rep_of l a := []]) ! rep_of (ufa_union l a b) c\<^sub>1) \<and> 
+rep_of (ufa_union l a b) e\<^sub>1 = rep_of (ufa_union l a b) c\<^sub>1 \<and> 
+rep_of (ufa_union l a b) e\<^sub>2 = rep_of (ufa_union l a b) c\<^sub>2"
+    by (metis ufa_union_aux nth_list_update_neq rep_of_ufa_union_invar use_list_invar_less_n_in_set(1,2))
+  with c c1_step c2_step CC_step have "eq' = F c\<^sub>1 c\<^sub>2 \<approx> c \<and>
+           c\<^sub>1 < length l \<and>
+           c\<^sub>2 < length l \<and>
+           c < length l \<and>
+           (rep_of l c\<^sub>1 \<noteq> rep_of l a \<longrightarrow>
+            contains_similar_equation
+             \<lparr>cc_list = ufa_union l a b, use_list = u[rep_of l a := []], lookup = t, pending = pe,
+                proof_forest = add_edge pf a b, pf_labels = add_label pfl pf a eq, input = ip\<rparr>
+             (rep_of l c\<^sub>1) c\<^sub>1 c\<^sub>2 c (u ! rep_of l a)) \<and>
+           (rep_of l c\<^sub>2 \<noteq> rep_of l a \<longrightarrow>
+            contains_similar_equation
+             \<lparr>cc_list = ufa_union l a b, use_list = u[rep_of l a := []], lookup = t, pending = pe,
+                proof_forest = add_edge pf a b, pf_labels = add_label pfl pf a eq, input = ip\<rparr>
+             (rep_of l c\<^sub>2) c\<^sub>1 c\<^sub>2 c (u ! rep_of l a))"
+    unfolding congruence_closure.select_convs 
+    by (metis (full_types) CC_d_c CC_e_c c_eq_b d(1) e(1) nth_list_update_neq)
+  then show "\<exists>c\<^sub>1 c\<^sub>2 c.
+              eq' = F c\<^sub>1 c\<^sub>2 \<approx> c \<and>
+              c\<^sub>1 < length l \<and>
+              c\<^sub>2 < length l \<and>
+              c < length l \<and>
+              (rep_of l c\<^sub>1 \<noteq> rep_of l a \<longrightarrow>
+               contains_similar_equation
+                \<lparr>cc_list = ufa_union l a b, use_list = u[rep_of l a := []], lookup = t, pending = pe,
+                   proof_forest = add_edge pf a b, pf_labels = add_label pfl pf a eq, input = ip\<rparr>
+                (rep_of l c\<^sub>1) c\<^sub>1 c\<^sub>2 c (u ! rep_of l a)) \<and>
+              (rep_of l c\<^sub>2 \<noteq> rep_of l a \<longrightarrow>
+               contains_similar_equation
+                \<lparr>cc_list = ufa_union l a b, use_list = u[rep_of l a := []], lookup = t, pending = pe,
+                   proof_forest = add_edge pf a b, pf_labels = add_label pfl pf a eq, input = ip\<rparr>
+                (rep_of l c\<^sub>2) c\<^sub>1 c\<^sub>2 c (u ! rep_of l a))" 
+    by blast
 qed
 
 lemma lookup_invar_step: 
   assumes "ufa_invar l" "a < length l" "b < length l" 
-"lookup_invar \<lparr>cc_list = l, use_list = u, lookup = t, pending = (eq # pe), proof_forest = pf, pf_labels = pfl, input = ip\<rparr>"
+    "lookup_invar \<lparr>cc_list = l, use_list = u, lookup = t, pending = (eq # pe), proof_forest = pf, pf_labels = pfl, input = ip\<rparr>"
     (is "lookup_invar ?base") 
     "use_list_invar \<lparr>cc_list = l, use_list = u, lookup = t, pending = (eq # pe), proof_forest = pf, pf_labels = pfl, input = ip\<rparr>"
     "length t = length l" "length u = length l"
@@ -959,15 +2065,15 @@ text \<open>All the equations in the pending list have valid variables, after a 
 
 lemma pending_invar_step:
   assumes "pending_invar \<lparr>cc_list = l, use_list = u, lookup = t, pending = (eq # pe), proof_forest = pf, pf_labels = pfl, input = ip\<rparr>" 
-(is "pending_invar ?base")    
-"lookup_invar \<lparr>cc_list = l, use_list = u, lookup = t, pending = (eq # pe), proof_forest = pf, pf_labels = pfl, input = ip\<rparr>"
+    (is "pending_invar ?base")    
+    "lookup_invar \<lparr>cc_list = l, use_list = u, lookup = t, pending = (eq # pe), proof_forest = pf, pf_labels = pfl, input = ip\<rparr>"
     "use_list_invar \<lparr>cc_list = l, use_list = u, lookup = t, pending = (eq # pe), proof_forest = pf, pf_labels = pfl, input = ip\<rparr>"
-"ufa_invar l" "a < length l" "b < length l" "length t = length l" "length u = length l"
-shows "pending_invar (propagate_step l u t pe pf pfl ip a b eq)"
-(is "pending_invar ?step") 
+    "ufa_invar l" "a < length l" "b < length l" "length t = length l" "length u = length l"
+  shows "pending_invar (propagate_step l u t pe pf pfl ip a b eq)"
+    (is "pending_invar ?step") 
   unfolding pending_invar_def
 proof(standard)+
-let ?mini_step = "\<lparr>cc_list = ufa_union l a b, 
+  let ?mini_step = "\<lparr>cc_list = ufa_union l a b, 
     use_list = u[rep_of l a := []], 
     lookup = t, 
     pending = pe,
@@ -979,18 +2085,18 @@ let ?mini_step = "\<lparr>cc_list = ufa_union l a b,
   from assms have 1: "pending_invar ?mini_step" 
     by (simp add: pending_invar_mini_step)
   from assms have 2: "lookup_invar ?mini_step" 
-  using lookup_invar_mini_step by blast
-from assms have 3: "use_list_invar ?mini_step" 
-  using use_list_invar_mini_step by presburger
+    using lookup_invar_mini_step by blast
+  from assms have 3: "use_list_invar ?mini_step" 
+    using use_list_invar_mini_step by presburger
   from assms have 4: "ufa_invar (ufa_union l a b)" 
-"length t = length (ufa_union l a b)"
-"length (u[rep_of l a := []]) = length (ufa_union l a b)"
-"a < length (ufa_union l a b)" "b < length (ufa_union l a b)"
+    "length t = length (ufa_union l a b)"
+    "length (u[rep_of l a := []]) = length (ufa_union l a b)"
+    "a < length (ufa_union l a b)" "b < length (ufa_union l a b)"
     using ufa_union_invar apply blast 
     by (simp_all add: assms)
   from assms use_list_invar_impl_valid_input_propagate_loop have "\<forall>j<length (u ! rep_of l a). use_list_valid_element ((u ! rep_of l a) ! j) (ufa_union l a b) 
 (rep_of l b)" "rep_of l b < length l"
-    apply blast
+     apply blast
     using assms(4) assms(6) rep_of_less_length_l by auto
   with  pending_invar_loop 1 2 3 4 assms  
   show "valid_vars_pending ((pending ?step) ! i) (cc_list ?step)"
@@ -998,20 +2104,20 @@ from assms have 3: "use_list_invar ?mini_step"
 qed
 
 lemma input_unchanged_loop:
-"input (propagate_loop a b cc) = 
+  "input (propagate_loop a b cc) = 
 input cc"
   apply(induction a b cc rule: propagate_loop.induct)
   by auto
- 
+
 lemma input_unchanged_step:
-"input (propagate_step l u t pe pf pfl ip a b eq) = ip"
+  "input (propagate_step l u t pe pf pfl ip a b eq) = ip"
   by (simp add: input_unchanged_loop)
 
 lemma use_list_invar_step: 
   assumes "ufa_invar l" "a < length l" "b < length l" 
-"use_list_invar \<lparr>cc_list = l, use_list = u, lookup = t, pending = (eq # pe), proof_forest = pf, pf_labels = pfl, input = ip\<rparr>"
+    "use_list_invar \<lparr>cc_list = l, use_list = u, lookup = t, pending = (eq # pe), proof_forest = pf, pf_labels = pfl, input = ip\<rparr>"
     (is "use_list_invar ?base") 
-  "length u = length l"
+    "length u = length l"
   shows "use_list_invar (propagate_step l u t pe pf pfl ip a b eq)" (is "use_list_invar ?step")
   unfolding use_list_invar_def 
 proof(standard, standard,standard, standard, standard)
@@ -1038,135 +2144,66 @@ qed
 
 lemma lookup_invar2_step:
   assumes 
-"lookup_invar2 \<lparr>cc_list = l, use_list = u, lookup = t, pending = (eq # pe), proof_forest = pf, pf_labels = pfl, input = ip\<rparr>"
-"use_list_invar2 \<lparr>cc_list = l, use_list = u, lookup = t, pending = (eq # pe), proof_forest = pf, pf_labels = pfl, input = ip\<rparr>"
-"use_list_invar \<lparr>cc_list = l, use_list = u, lookup = t, pending = (eq # pe), proof_forest = pf, pf_labels = pfl, input = ip\<rparr>"
-"lookup_invar \<lparr>cc_list = l, use_list = u, lookup = t, pending = (eq # pe), proof_forest = pf, pf_labels = pfl, input = ip\<rparr>"
-"pending_invar \<lparr>cc_list = l, use_list = u, lookup = t, pending = (eq # pe), proof_forest = pf, pf_labels = pfl, input = ip\<rparr>"
-"ufa_invar l"  "length u = length l" "length t = length l"
-"a < length l" "b < length l" "rep_of l a \<noteq> rep_of l b"
-"a = left eq" "b = right eq"
+    "lookup_invar2 \<lparr>cc_list = l, use_list = u, lookup = t, pending = (eq # pe), proof_forest = pf, pf_labels = pfl, input = ip\<rparr>"
+    "use_list_invar2 \<lparr>cc_list = l, use_list = u, lookup = t, pending = (eq # pe), proof_forest = pf, pf_labels = pfl, input = ip\<rparr>"
+    "use_list_invar \<lparr>cc_list = l, use_list = u, lookup = t, pending = (eq # pe), proof_forest = pf, pf_labels = pfl, input = ip\<rparr>"
+    "lookup_invar \<lparr>cc_list = l, use_list = u, lookup = t, pending = (eq # pe), proof_forest = pf, pf_labels = pfl, input = ip\<rparr>"
+    "pending_invar \<lparr>cc_list = l, use_list = u, lookup = t, pending = (eq # pe), proof_forest = pf, pf_labels = pfl, input = ip\<rparr>"
+    "ufa_invar l"  "length u = length l" "length t = length l"
+    "a < length l" "b < length l" "rep_of l a \<noteq> rep_of l b"
+    "a = left eq" "b = right eq"
 shows "lookup_invar2 (propagate_step l u t pe pf pfl ip a b eq)"
-  using assms proof(induction "rep_of l b" "u ! rep_of l a" 
-   "\<lparr>cc_list = ufa_union l a b, 
+proof-
+  let ?base = "\<lparr>cc_list = l, use_list = u, lookup = t, pending = eq # pe, proof_forest = pf, pf_labels = pfl,
+               input = ip\<rparr>"
+  let ?mini_step = "
+     \<lparr>cc_list = ufa_union l a b, use_list = u[rep_of l a := []], lookup = t, pending = pe,
+        proof_forest = add_edge pf a b, pf_labels = add_label pfl pf a eq, input = ip\<rparr>"
+  have 1: "lookup_invar2' ?mini_step (u ! rep_of l a)" 
+    using assms lookup_invar2_mini_step by blast 
+  have 2: "\<forall> eq' \<in> set (u ! rep_of l a) . 
+(\<exists> c\<^sub>1 c\<^sub>2 c . eq' = (F c\<^sub>1 c\<^sub>2 \<approx> c) \<and> c\<^sub>1 < length l \<and> c\<^sub>2 < length l \<and> c < length l
+\<and> (rep_of l c\<^sub>1 \<noteq> rep_of l a \<longrightarrow> 
+contains_similar_equation \<lparr>cc_list = ufa_union l a b, 
     use_list = u[rep_of l a := []], 
     lookup = t, 
     pending = pe,
     proof_forest = add_edge pf a b, 
     pf_labels = add_label pfl pf a eq, 
-    input = ip\<rparr>" rule: propagate_loop.induct)
-  case (1 u1 urest l u t pe pf pfl ip)
-  then show ?case sorry
-next
-  case 2
-  show ?case unfolding lookup_invar2_def 2(1)[symmetric] propagate_loop.simps congruence_closure.select_convs
-  proof(standard, standard, standard, standard, standard, standard, standard, standard, standard, standard)
-    fix a' b' c c\<^sub>1 c\<^sub>2
-    assume prems: "a' < length (ufa_union l a b)" "b' < length (ufa_union l a b)"
-"ufa_union l a b ! a' = a'" "ufa_union l a b ! b' = b'"
-"t ! a' ! b' = Some (F c\<^sub>1 c\<^sub>2 \<approx> c)"
-    with 2(3) have *: "l ! a' = a'" "l ! b' = b'" "a' < length l" "b' < length l"
-"t ! a' ! b' = Some (F c\<^sub>1 c\<^sub>2 \<approx> c)"
-      using assms ufa_union_root apply blast+ 
-      using prems by auto
-    with 2(2) obtain b\<^sub>1 b\<^sub>2 bc a\<^sub>1 a\<^sub>2 ac where 1: "
-         (F b\<^sub>1 b\<^sub>2 \<approx> bc) \<in> set (u ! b') \<and>
-         rep_of l b\<^sub>1 = rep_of l c\<^sub>1 \<and>
-         rep_of l b\<^sub>2 = rep_of l c\<^sub>2 \<and>
-         Congruence_Closure
-          (representativeE
-            \<lparr>cc_list = l, use_list = u, lookup = t, pending = eq # pe, proof_forest = pf,
-               pf_labels = pfl, input = ip\<rparr> \<union>
-           pending_set (eq # pe))
-          (bc \<approx> c)"
-     "
-         (F a\<^sub>1 a\<^sub>2 \<approx> ac) \<in> set (u ! a') \<and>
-         rep_of l a\<^sub>1 = rep_of l c\<^sub>1 \<and>
-         rep_of l a\<^sub>2 = rep_of l c\<^sub>2 \<and>
-         Congruence_Closure
-          (representativeE
-            \<lparr>cc_list = l, use_list = u, lookup = t, pending = eq # pe, proof_forest = pf,
-               pf_labels = pfl, input = ip\<rparr> \<union>
-           pending_set (eq # pe))
-          (ac \<approx> c)" unfolding lookup_invar2_def congruence_closure.select_convs
-      by blast
-    from 2(1) have 3: "u[rep_of l a := []] = u" 
-      by (metis list_update_id)
-    have 4: "aa < length l \<Longrightarrow> bb < length l \<Longrightarrow> rep_of l aa = rep_of l bb \<Longrightarrow> rep_of (ufa_union l a b) aa = rep_of (ufa_union l a b) bb" 
-      for aa bb using assms rep_of_ufa_union_invar by blast
-    from 2(4) use_list_invar_less_n_in_set * 1
-    have 5: "b\<^sub>1 < length l" "b\<^sub>2 < length l" "bc < length l"
-"a\<^sub>1 < length l" "a\<^sub>2 < length l" "ac < length l"
-      by metis+
-    from inv2_mini_step[OF assms(6,9,10,12,13,2,1,5,4)] 2(1)
- assms have 6: "Congruence_Closure
-          (representativeE
-            \<lparr>cc_list = l, use_list = u, lookup = t, pending = eq # pe, proof_forest = pf,
-               pf_labels = pfl, input = ip\<rparr> \<union>
-           pending_set (eq # pe)) 
-= Congruence_Closure
-         (representativeE
-              \<lparr>cc_list = ufa_union l a b, use_list = u[rep_of l a := []], lookup = t, pending = pe,
-                 proof_forest = add_edge pf a b, pf_labels = add_label pfl pf a eq, input = ip\<rparr> \<union>
-             pending_set pe)" 
-      by force
-    from assms(4) * have "c\<^sub>1 < length l" "c\<^sub>2 < length l" "c < length l"
-      unfolding lookup_invar_def 
-      by fastforce+
-    with 1 3 4 5 6 * have "
-           ((F b\<^sub>1 b\<^sub>2 \<approx> bc) \<in> set (u[rep_of l a := []] ! b') \<and>
-           rep_of (ufa_union l a b) b\<^sub>1 = rep_of (ufa_union l a b) c\<^sub>1 \<and>
-           rep_of (ufa_union l a b) b\<^sub>2 = rep_of (ufa_union l a b) c\<^sub>2 \<and>
-           Congruence_Closure
-            (representativeE
-              \<lparr>cc_list = ufa_union l a b, use_list = u[rep_of l a := []], lookup = t, pending = pe,
-                 proof_forest = add_edge pf a b, pf_labels = add_label pfl pf a eq, input = ip\<rparr> \<union>
-             pending_set pe)
-            (bc \<approx> c))
-       ""
-           (F a\<^sub>1 a\<^sub>2 \<approx> ac) \<in> set (u[rep_of l a := []] ! a') \<and>
-           rep_of (ufa_union l a b) a\<^sub>1 = rep_of (ufa_union l a b) c\<^sub>1 \<and>
-           rep_of (ufa_union l a b) a\<^sub>2 = rep_of (ufa_union l a b) c\<^sub>2 \<and>
-           Congruence_Closure
-            (representativeE
-              \<lparr>cc_list = ufa_union l a b, use_list = u[rep_of l a := []], lookup = t, pending = pe,
-                 proof_forest = add_edge pf a b, pf_labels = add_label pfl pf a eq, input = ip\<rparr> \<union>
-             pending_set pe)
-            (ac \<approx> c)" unfolding 6 3 
-      by blast+
-    then show "(\<exists>b\<^sub>1 b\<^sub>2 ba.
-           (F b\<^sub>1 b\<^sub>2 \<approx> ba) \<in> set (u[rep_of l a := []] ! a') \<and>
-           rep_of (ufa_union l a b) b\<^sub>1 = rep_of (ufa_union l a b) c\<^sub>1 \<and>
-           rep_of (ufa_union l a b) b\<^sub>2 = rep_of (ufa_union l a b) c\<^sub>2 \<and>
-           Congruence_Closure
-            (representativeE
-              \<lparr>cc_list = ufa_union l a b, use_list = u[rep_of l a := []], lookup = t, pending = pe,
-                 proof_forest = add_edge pf a b, pf_labels = add_label pfl pf a eq, input = ip\<rparr> \<union>
-             pending_set pe)
-            (ba \<approx> c)) \<and>
-       (\<exists>b\<^sub>1 b\<^sub>2 ba.
-           (F b\<^sub>1 b\<^sub>2 \<approx> ba) \<in> set (u[rep_of l a := []] ! b') \<and>
-           rep_of (ufa_union l a b) b\<^sub>1 = rep_of (ufa_union l a b) c\<^sub>1 \<and>
-           rep_of (ufa_union l a b) b\<^sub>2 = rep_of (ufa_union l a b) c\<^sub>2 \<and>
-           Congruence_Closure
-            (representativeE
-              \<lparr>cc_list = ufa_union l a b, use_list = u[rep_of l a := []], lookup = t, pending = pe,
-                 proof_forest = add_edge pf a b, pf_labels = add_label pfl pf a eq, input = ip\<rparr> \<union>
-             pending_set pe)
-            (ba \<approx> c))"
-      by blast
-  qed
+    input = ip\<rparr> (rep_of l c\<^sub>1) c\<^sub>1 c\<^sub>2 c (u ! rep_of l a))
+
+\<and> 
+(rep_of l c\<^sub>2 \<noteq> rep_of l a \<longrightarrow> 
+contains_similar_equation \<lparr>cc_list = ufa_union l a b, 
+    use_list = u[rep_of l a := []], 
+    lookup = t, 
+    pending = pe,
+    proof_forest = add_edge pf a b, 
+    pf_labels = add_label pfl pf a eq, 
+    input = ip\<rparr> (rep_of l c\<^sub>2) c\<^sub>1 c\<^sub>2 c (u ! rep_of l a))
+)" using assms lookup2_invar_impl_valid_input_propagate_loop by blast
+  then have 
+    3: "\<forall>j<length (u ! rep_of l a). use_list_valid_element (u ! rep_of l a ! j) (ufa_union l a b) (rep_of l b)"
+    "rep_of l b < length l"  using assms use_list_invar_impl_valid_input_propagate_loop 
+    by simp_all
+  have 4: "use_list_invar ?mini_step" "lookup_invar ?mini_step" 
+    using assms use_list_invar_mini_step lookup_invar_mini_step by auto
+  have 5: "\<forall>j<length (u ! rep_of l a). use_list_valid_element (u ! rep_of l a ! j) l (rep_of l a)"
+    using assms unfolding use_list_invar_def congruence_closure.select_convs
+    using rep_of_less_length_l rep_of_root by auto
+  from lookup_invar2_loop[OF assms(6,9,10,11) 1 2 3 4 _ _ _ 5] show ?thesis 
+    by (metis assms(7) assms(8) length_list_update)
 qed
 
 lemma inv2_invar_step:
   assumes "cc_invar \<lparr>cc_list = l, use_list = u, lookup = t, pending = (eq # pe), proof_forest = pf, pf_labels = pfl, input = ip\<rparr>"
-"use_list_invar2 \<lparr>cc_list = l, use_list = u, lookup = t, pending = (eq # pe), proof_forest = pf, pf_labels = pfl, input = ip\<rparr>"
-"lookup_invar2 \<lparr>cc_list = l, use_list = u, lookup = t, pending = (eq # pe), proof_forest = pf, pf_labels = pfl, input = ip\<rparr>"
-"a < length l" "b < length l" "rep_of l a \<noteq> rep_of l b"
-"a = left eq" "b = right eq"
-shows "inv2 (propagate_step l u t pe pf pfl ip a b eq)" 
+    "use_list_invar2 \<lparr>cc_list = l, use_list = u, lookup = t, pending = (eq # pe), proof_forest = pf, pf_labels = pfl, input = ip\<rparr>"
+    "lookup_invar2 \<lparr>cc_list = l, use_list = u, lookup = t, pending = (eq # pe), proof_forest = pf, pf_labels = pfl, input = ip\<rparr>"
+    "a < length l" "b < length l" "rep_of l a \<noteq> rep_of l b"
+    "a = left eq" "b = right eq"
+  shows "inv2 (propagate_step l u t pe pf pfl ip a b eq)" 
 proof-
-let ?mini_step = "\<lparr>cc_list = ufa_union l a b, 
+  let ?mini_step = "\<lparr>cc_list = ufa_union l a b, 
     use_list = u[rep_of l a := []], 
     lookup = t, 
     pending = pe,
@@ -1184,23 +2221,23 @@ let ?mini_step = "\<lparr>cc_list = ufa_union l a b,
     using assms(1,4,5) lookup_invar_mini_step apply blast
     using assms(1,4,5) use_list_invar_mini_step lengths invar apply presburger
     using assms unfolding cc_list_invar_def by (simp add: ufa_union_invar)
-from inv2_mini_step assms invar have base: "Congruence_Closure (representativeE ?mini_step
+  from inv2_mini_step assms invar have base: "Congruence_Closure (representativeE ?mini_step
 \<union> pending_set pe
 \<union> set (u ! rep_of l a)) = 
 Congruence_Closure 
 (representativeE 
 \<lparr>cc_list = l, use_list = u, lookup = t, pending = (eq # pe), proof_forest = pf, pf_labels = pfl, input = ip\<rparr>
 \<union> pending_set (eq # pe))" 
-  by blast
+    by blast
   have 
-"\<forall>j<length (u ! rep_of l a). use_list_valid_element (u ! rep_of l a ! j) (ufa_union l a b) (rep_of l b)"
-"rep_of l b < length l" 
+    "\<forall>j<length (u ! rep_of l a). use_list_valid_element (u ! rep_of l a ! j) (ufa_union l a b) (rep_of l b)"
+    "rep_of l b < length l" 
     using invar use_list_invar_impl_valid_input_propagate_loop[OF invar assms(4,5)] assms(1)
      apply blast
     by (simp add: assms(4,5) invar rep_of_less_length_l)
   with inv2_loop[of "a"
-"?mini_step"
-b "u ! rep_of l a" "rep_of l b"] assms use_list_invar_impl_valid_input_propagate_loop 
+      "?mini_step"
+      b "u ! rep_of l a" "rep_of l b"] assms use_list_invar_impl_valid_input_propagate_loop 
   have *: "Congruence_Closure (representativeE \<lparr>cc_list = ufa_union l a b, 
     use_list = u[rep_of l a := []], 
     lookup = t, 
@@ -1238,7 +2275,7 @@ lemma propagate_preserves_length_cc_list:
   shows "nr_vars (propagate cc) = nr_vars cc"
   using assms apply(induction rule: propagate.pinduct)
   unfolding propagate.psimps Let_def
-  apply simp using assms sorry
+   apply simp using assms sorry
 
 lemma propagate_preserves_length_use_list:
   assumes "propagate_dom cc" "length (use_list cc) = n"
@@ -1327,12 +2364,12 @@ qed
 
 lemma propagate_preserves_length_pf_labels:
   assumes "propagate_dom cc" "length (pf_labels cc) = nr_vars cc" 
-"length (proof_forest cc) = nr_vars cc" "ufa_invar (proof_forest cc)"
-"pending_invar cc" "inv_same_rep_classes cc" "ufa_invar (cc_list cc)"
-"nr_vars cc = length (use_list cc)"
-"nr_vars cc = length (lookup cc)"
-"lookup_invar cc" "use_list_invar cc"
-shows "length (pf_labels (propagate cc)) = nr_vars cc"
+    "length (proof_forest cc) = nr_vars cc" "ufa_invar (proof_forest cc)"
+    "pending_invar cc" "inv_same_rep_classes cc" "ufa_invar (cc_list cc)"
+    "nr_vars cc = length (use_list cc)"
+    "nr_vars cc = length (lookup cc)"
+    "lookup_invar cc" "use_list_invar cc"
+  shows "length (pf_labels (propagate cc)) = nr_vars cc"
   using assms proof(induction rule: propagate.pinduct)
   case (1 l u t pf pfl ip)
   then show ?case 
@@ -1355,7 +2392,7 @@ next
       using 2 a_def b_def pending_invar_Cons propagate.psimps(2) unfolding Let_def sorry
   next
     case False
-    (*then have rep_pf: "rep_of pf a \<noteq> rep_of pf b" 
+      (*then have rep_pf: "rep_of pf a \<noteq> rep_of pf b" 
       using "2.prems"(5) a_b inv_same_rep_classes_divided by auto
     with add_edge_domain "2.prems" a_b have "add_edge_dom (pf, a, b)" 
       by (metis congruence_closure.select_convs(4))
@@ -1391,35 +2428,35 @@ qed
 
 lemma length_propagate_cc:
   assumes "cc_invar cc"
- "propagate_dom cc"
+    "propagate_dom cc"
   shows "nr_vars cc = nr_vars (propagate cc)"
-  "nr_vars cc = length (use_list (propagate cc))"
-  "nr_vars cc = length (lookup (propagate cc))"
-  "nr_vars cc = length (proof_forest (propagate cc))"
-  "nr_vars cc = length (pf_labels (propagate cc))"
+    "nr_vars cc = length (use_list (propagate cc))"
+    "nr_vars cc = length (lookup (propagate cc))"
+    "nr_vars cc = length (proof_forest (propagate cc))"
+    "nr_vars cc = length (pf_labels (propagate cc))"
   using assms propagate_preserves_length_use_list propagate_preserves_length_cc_list inv_same_length_def propagate_preserves_length_lookup
-  cc_list_invar_def propagate_preserves_length_proof_forest propagate_preserves_length_pf_labels proof_forest_invar_def 
+    cc_list_invar_def propagate_preserves_length_proof_forest propagate_preserves_length_pf_labels proof_forest_invar_def 
   by auto 
 
 lemma inv_same_length_step:
   assumes "cc_invar \<lparr>cc_list = l, use_list = u, lookup = t, pending = (eq # pe), proof_forest = pf, pf_labels = pfl, input = ip\<rparr>"
-"rep_of l a \<noteq> rep_of l b" "a = left eq" "b = right eq"
-shows "inv_same_length (propagate_step l u t pe pf pfl ip a b eq)
+    "rep_of l a \<noteq> rep_of l b" "a = left eq" "b = right eq"
+  shows "inv_same_length (propagate_step l u t pe pf pfl ip a b eq)
 (nr_vars (propagate_step l u t pe pf pfl ip a b eq))" 
 proof-
   from assms have pe_valid: "valid_vars_pending eq (length l)" 
     using pending_invar_Cons by auto
   show ?thesis unfolding inv_same_length_def
-  apply(rule conjI)+
-      apply blast
-  using assms inv_same_length_def apply fastforce
-  using assms inv_same_length_def  apply auto[1]
-  using assms add_edge_preserves_length' pe_valid pending_left_right_valid' inv_same_rep_classes_divided length_list_update
-  unfolding inv_same_length_def proof_forest_invar_def subgoal sorry
-  (*apply (metis congruence_closure.select_convs(1) congruence_closure.select_convs(4))*)
-  using assms add_label_preserves_length add_label_domain pending_left_right_valid' 
-  unfolding proof_forest_invar_def inv_same_length_def 
-  by auto
+    apply(rule conjI)+
+    apply blast
+    using assms inv_same_length_def apply fastforce
+    using assms inv_same_length_def  apply auto[1]
+    using assms add_edge_preserves_length' pe_valid pending_left_right_valid' inv_same_rep_classes_divided length_list_update
+    unfolding inv_same_length_def proof_forest_invar_def subgoal sorry
+        (*apply (metis congruence_closure.select_convs(1) congruence_closure.select_convs(4))*)
+    using assms add_label_preserves_length add_label_domain pending_left_right_valid' 
+    unfolding proof_forest_invar_def inv_same_length_def 
+    by auto
 qed
 
 subsection \<open>cc_invar lemmata\<close>
@@ -1432,7 +2469,7 @@ proof(rule conjI)+
   proof(standard, standard, standard, standard, standard)
     fix i j 
     assume "i < nr_vars (initial_cc n)" "j < length (use_list (initial_cc n) ! i)"
-"cc_list (initial_cc n) ! i = i"
+      "cc_list (initial_cc n) ! i = i"
     then have "length (use_list (initial_cc n) ! i) = 0" 
       by fastforce
     then have "False" 
@@ -1442,7 +2479,7 @@ proof(rule conjI)+
   proof(standard, standard, standard, standard, standard, standard, standard)
     fix i j
     assume "i < nr_vars (initial_cc n)" "j < nr_vars (initial_cc n)"
-"cc_list (initial_cc n) ! i = i \<and> cc_list (initial_cc n) ! j = j"
+      "cc_list (initial_cc n) ! i = i \<and> cc_list (initial_cc n) ! j = j"
     then show "lookup (initial_cc n) ! i ! j = None" 
       by force
   next
@@ -1466,7 +2503,7 @@ proof(rule conjI)+
   proof(standard, standard, standard, standard)
     fix i j
     assume "i < length (proof_forest (initial_cc n))"
-"j < length (proof_forest (initial_cc n))"
+      "j < length (proof_forest (initial_cc n))"
     then show "(rep_of (cc_list (initial_cc n)) i =
             rep_of (cc_list (initial_cc n)) j) =
            (rep_of (proof_forest (initial_cc n)) i =
@@ -1481,8 +2518,8 @@ qed
 
 lemma cc_invar_step:
   assumes "cc_invar_pending \<lparr>cc_list = l, use_list = u, lookup = t, proof_forest = pf, pf_labels = pfl, input = ip\<rparr> (pe # xs)"
-"valid_vars_pending pe (length l)" "a = left pe" "b = right pe" "rep_of l a \<noteq> rep_of l b"
-shows "cc_invar_pending (propagate_step l u t pf pfl ip a b pe) xs"
+    "valid_vars_pending pe (length l)" "a = left pe" "b = right pe" "rep_of l a \<noteq> rep_of l b"
+  shows "cc_invar_pending (propagate_step l u t pf pfl ip a b pe) xs"
   apply (rule conjI)+
   using assms cc_list_invar_def pending_left_right_valid' ufa_union_invar apply auto[1]
   using assms cc_list_invar_def inv_same_length_def pending_left_right_valid' use_list_invar_step apply auto[1]
